add init functions; prove init for skiplist

templates/lockfree/node_impl2.v
@@ -9,7 +9,7 @@ From iris.bi.lib Require Import fractional.
 From flows Require Export flows array_util node_module bool_ra gset_seq.
 Set Default Proof Using "All".
 
-Module IMPL1 : NODE_IMPL.
+Module IMPL2 : NODE_IMPL.
 
   Parameter L : nat. (* Maximum Height *)
   Parameter W : nat. (* Keyspace *)
@@ -26,8 +26,7 @@ Module IMPL1 : NODE_IMPL.
       if: #L ≤ "i" then
         #()
       else
-        let: "li" := ref (#false, #l0) in
-        ("arr" +ₗ "i") <- "li";;
+        ("arr" +ₗ "i") <- InjR #l0;;
         "cT" ("i" + #1) "arr".
 
   Definition createTail : val :=
@@ -37,14 +36,13 @@ Module IMPL1 : NODE_IMPL.
       ("tl" +ₗ #1) <- "arr";;
       createTail_rec #0%nat "arr";;
       "tl".
-
+  
   Definition createHead_rec : val :=
     rec: "cH" "i" "arr" "tl" :=
       if: #L ≤ "i" then
         #()
       else
-        let: "li" := ref (#false, "tl") in
-        ("arr" +ₗ "i") <- "li";;
+        ("arr" +ₗ "i") <- InjR "tl";;
         "cH" ("i" + #1) "arr" "tl".
 
   Definition createHead : val :=
@@ -61,8 +59,7 @@ Module IMPL1 : NODE_IMPL.
         #()
       else
         let: "si" := !("succs" +ₗ "i") in
-        let: "li" := ref (#false, "si") in 
-        ("arr" +ₗ "i") <- "li";;
+        ("arr" +ₗ "i") <- InjR "si";;
         "cN" ("i" + #1) "h" "arr" "succs".
 
   Definition createNode : val :=
@@ -73,11 +70,11 @@ Module IMPL1 : NODE_IMPL.
       ("n" +ₗ #1) <- "arr";;
       createNode_rec #0%nat "h" "arr" "succs";;
       "n".
-
+  
   Definition getKey : val :=
     λ: "n",
       Fst (! "n").
-
+  
   Definition getHeight : val :=
     λ: "n",
       Snd (! "n").
@@ -85,87 +82,82 @@ Module IMPL1 : NODE_IMPL.
   Definition findNext : val :=
     λ: "n" "i",
       let: "arr" := ! ("n" +ₗ #1) in
-      let: "li" := ! ("arr" +ₗ "i") in
-      let: "res" := ! "li" in
-      "res".
+      let: "res" := ! ("arr" +ₗ "i") in
+      match: "res" with
+        InjL "l" => (#true, "l")
+      | InjR "l" => (#false, "l") end.
   
   Definition markNode : val :=
     rec: "markN" "n" "i" :=
       let: "arr" := ! ("n" +ₗ #1) in
-      let: "li" := ! ("arr" +ₗ "i") in
-      let: "res" := ! "li" in
-      if: (Fst "res") then
-        NONEV
-      else
-        let: "new" := ref (#true, Snd "res") in
-        if: CAS ("arr" +ₗ "i") "li" "new" then
-          (InjRV #())
+      let: "res" := ! ("arr" +ₗ "i") in
+      match: "res" with
+        InjL "l" => NONEV
+      | InjR "l" => 
+        if: CAS ("arr" +ₗ "i") (InjR "l") (InjL "l") then
+          InjRV #()
         else
-          "markN" "n" "i".
+          "markN" "n" "i"
+      end.
 
-  Definition markNode' : val := 
+  Definition markNode' : val :=
     rec: "markN" "n" "p" :=
       let: "arr" := ! ("n" +ₗ #1) in
-      let: "li" := ! ("arr" +ₗ #0%nat) in
-      let: "res" := ! "li" in
-      if: (Fst "res") then
-        NONEV
-      else
-        let: "new" := ref (#true, Snd "res") in
-        let: "res" := Resolve (CmpXchg ("arr" +ₗ #0%nat) "li" "new") "p" #() in
+      let: "res" := ! ("arr" +ₗ #0%nat) in
+      match: "res" with
+        InjL "l" => NONEV
+      | InjR "l" => 
+        let: "res" := Resolve (CmpXchg ("arr" +ₗ #0%nat) (InjR "l") (InjL "l")) "p" #() in
         if: Snd "res" then
-          (InjRV #())
+          InjRV #()
         else
-          "markN" "n" "p".
-          
+          "markN" "n" "p"
+      end.
+
   Definition changeNext : val :=
     rec: "chN" "n" "m" "m'" "i" :=
       let: "arr" := ! ("n" +ₗ #1) in
-      let: "li" := ! ("arr" +ₗ "i") in
-      let: "res" := ! "li" in
-      if: (Fst "res") then
-        NONEV
-      else
-        if: (Snd "res") = "m" then
-          let: "new" := ref (#false, "m'") in
-          if: CAS ("arr" +ₗ "i") "li" "new" then
-            (InjRV #())
+      let: "res" := ! ("arr" +ₗ "i") in
+      match: "res" with
+        InjL "l" => NONEV
+      | InjR "l" =>
+        if: CAS ("arr" +ₗ "i") (InjR "m") (InjR "m'") then
+            InjRV #()
           else
             "chN" "n" "m" "m'" "i"
-        else
-          NONEV.
+      end.
 
   Definition changeNext' : val :=
     rec: "chN" "n" "m" "m'" "p" :=
       let: "arr" := ! ("n" +ₗ #1) in
-      let: "li" := ! ("arr" +ₗ #0%nat) in
-      let: "res" := ! "li" in
-      if: (Fst "res") then
-        NONEV
-      else
-        if: (Snd "res") = "m" then
-          let: "new" := ref (#false, "m'") in
-          let: "res" := Resolve (CmpXchg ("arr" +ₗ #0%nat) "li" "new") "p" #() in
-          if: Snd "res" then
-            (InjRV #())
+      let: "res" := ! ("arr" +ₗ #0%nat) in
+      match: "res" with
+        InjL "l" => NONEV
+      | InjR "l" =>
+        let: "res" := Resolve (CmpXchg ("arr" +ₗ #0%nat) (InjR "m") (InjR "m'")) "p" #() in
+        if: Snd "res" then
+            InjRV #()
           else
             "chN" "n" "m" "m'" "p"
-        else
-          NONEV.
+      end.
 
   (* Context `{!heapGS Σ}. *)
   (* Notation iProp := (iProp Σ). *)
 
+
   Definition node Σ (Hg1 : heapGS Σ) (n: Node) (h: nat) (mark: MarkT) (next: NextT) 
     (k: nat) : iProp Σ :=
-    ∃ (arr: loc) (ls: list loc),
+    ∃ (arr: loc) (vs: list val),
        n ↦□ (#k, #h)
     ∗ (n +ₗ 1) ↦□ #arr
-    ∗ arr ↦∗ ((fun l => # (LitLoc l)) <$> ls)
-    ∗ ⌜length ls = h ∧ 0 < h⌝
-    ∗ ∀ (l: loc) (i: nat), ⌜ls !! i = Some l⌝ -∗
-        l ↦□ (#((mark !!! i): bool), #((next !!! i: loc))).
-  
+    ∗ arr ↦∗ vs
+    ∗ ⌜length vs = h ∧ 0 < h⌝
+    ∗ ∀ (v: val) (i: nat), ⌜vs !! i = Some v⌝ -∗
+        (⌜match v with 
+          | InjLV #(LitLoc l) => mark !!! i = true ∧ next !!! i = l
+          | InjRV #(LitLoc l) => mark !!! i = false ∧ next !!! i = l
+          | _ => False end⌝).
+
   Global Instance node_timeless_proof : ∀ Σ Hg1 n h mark next k, 
         Timeless (node Σ Hg1 n h mark next k).
   Proof. try apply _. Qed.
@@ -179,10 +171,10 @@ Module IMPL1 : NODE_IMPL.
     iDestruct (mapsto_agree with "Hn0 Hn1") as "%H'". inversion H'. clear H'.
     iDestruct (mapsto_agree with "Hk0 Hk1") as "%H'". inversion H'. clear H'.
     assert (∃ l0 ls0', ls0 = l0 :: ls0') as [l0 [ls0' Def_ls0]].
-    { destruct ls0. rewrite /= in Len_vs0. lia. by exists l, ls0. }
+    { destruct ls0. rewrite /= in Len_vs0. lia. by exists v, ls0. }
     rewrite Def_ls0 array_cons. iDestruct "Harr0" as "(Harr0 & Harr0')". 
     assert (∃ l1 ls1', ls1 = l1 :: ls1') as [l1 [ls1' Def_ls1]].
-    { destruct ls1. rewrite /= in Len_vs1. lia. by exists l, ls1. }
+    { destruct ls1. rewrite /= in Len_vs1. lia. by exists v, ls1. }
     rewrite Def_ls1 array_cons. iDestruct "Harr1" as "(Harr1 & Harr1')".
     iCombine "Harr0 Harr1" as "H'". iPoseProof (mapsto_valid with "H'") as "%".
     exfalso; try done.
@@ -255,51 +247,43 @@ Module IMPL1 : NODE_IMPL.
       rewrite elem_of_dom H''. done.
   Qed.
 
-  Lemma createTail_rec_spec Σ (Hg1 : heapGS Σ) (arr: loc) (ls : list Node) (i: nat) :
-  ⊢  {{{ arr ↦∗ ((fun l => # (LitLoc l)) <$> ls)
-         ∗ ⌜length ls = L⌝
-         ∗ ∀ (l: loc) (j: nat), 
-           ⌜ls !! j = Some l⌝ -∗ ⌜j < i⌝ -∗
-             l ↦□ (#false, #l0) }}}
-           createTail_rec #i #arr
-      {{{ (ls': list Node),
-          RET #();
-              arr ↦∗ ((fun l => # (LitLoc l)) <$> ls')
-            ∗ ⌜length ls' = L⌝
-            ∗ ∀ (l: loc) (j: nat), 
-              ⌜ls' !! j = Some l⌝ -∗ ⌜j < L⌝ -∗
-                l ↦□ (#false, #l0) }}}.
+  Lemma createTail_rec_spec Σ (Hg1 : heapGS Σ) (arr: loc) (vs: list val) (i: nat) :
+  ⊢ {{{  arr ↦∗ vs
+         ∗ ⌜length vs = L⌝
+         ∗ ∀ (v: val) (j: nat), 
+            ⌜vs !! j = Some v⌝ -∗ ⌜j < i⌝ -∗
+              (⌜match v with 
+              | InjRV #(LitLoc l) => l = l0
+              | _ => False end⌝) }}}
+          createTail_rec #i #arr
+    {{{ (vs': list val),
+        RET #();
+            arr ↦∗ vs'
+          ∗ ⌜length vs' = L⌝
+          ∗ ∀ (v: val) (j: nat), 
+            ⌜vs' !! j = Some v⌝ -∗ ⌜j < L⌝ -∗
+              (⌜match v with 
+              | InjRV #(LitLoc l) => l = l0
+              | _ => False end⌝) }}}.
   Proof.
-    iIntros (Φ) "!> Hpre Hpost". iLöb as "IH" forall (i ls).
-    iDestruct "Hpre" as "(Harr & %Len_ls & Hls)".
+    iIntros (Φ) "!> Hpre Hpost". iLöb as "IH" forall (i vs).
+    iDestruct "Hpre" as "(Harr & %Len_ls & Hvs)".
     wp_lam. wp_pures. destruct (bool_decide (L ≤ i)%Z) eqn: Hi; wp_pures.
-    - iApply ("Hpost" $! ls). iFrame. iSplitR; first by iPureIntro.
-      iModIntro. iIntros (l j)"%Hlj %j_le_L".
-      rewrite bool_decide_eq_true in Hi. iApply "Hls"; try done.
+    - iApply ("Hpost" $! vs). iFrame. iSplitR; first by iPureIntro.
+      iModIntro. iIntros (v j)"%Hvj %j_le_h".
+      rewrite bool_decide_eq_true in Hi. iApply "Hvs"; try done.
       iPureIntro; lia.
-    - rewrite bool_decide_eq_false in Hi.
-      wp_apply wp_alloc; try done.
-      iIntros (l)"(Hl&_)". wp_pures. wp_bind (_ <- _)%E.
-      iApply fupd_wp. iDestruct (mapsto_persist with "Hl") as ">#Hl". iModIntro.
-      iApply (wp_store_offset _ _ arr i with "Harr").
-      { apply lookup_lt_is_Some_2. rewrite fmap_length Len_ls. lia. }
+    - rewrite bool_decide_eq_false in Hi. 
+      wp_bind (_ <- _)%E. iApply (wp_store_offset _ _ arr i vs with "Harr").
+      { apply lookup_lt_is_Some_2. lia. }
       iIntros "!> Harr". wp_pures.
       assert (Z.add i 1 = (i+1)%nat) as -> by lia. 
-      iSpecialize ("IH" $! (i+1) (<[i:=l]>ls)).
-      iApply ("IH" with "[Harr Hls]"); try done.
-      assert ((λ l0 : loc, #l0) <$> <[i:=l]> ls = 
-                  <[i:=#l]> ((λ l0 : loc, #l0) <$> ls)) as ->.
-      { apply list_eq. intros i'. 
-        destruct (decide (i' = i)) as [-> | Hi'].
-        rewrite list_lookup_fmap !list_lookup_insert /=. done.
-        rewrite Len_ls; lia. rewrite fmap_length Len_ls. lia.
-        rewrite list_lookup_fmap !list_lookup_insert_ne /=; try done.
-        by rewrite list_lookup_fmap. }
+      iSpecialize ("IH" $! (i+1) (<[i:= InjRV #l0]>vs)).
+      iApply ("IH" with "[Harr Hvs]"); try done.
       iFrame "Harr". iSplitR. { iPureIntro. by rewrite insert_length. }
-      iIntros (l' j)"%Hlj %Hj". destruct (decide (j = i)) as [-> | Hij].
-      { rewrite list_lookup_insert in Hlj. inversion Hlj. subst l'.
-        iFrame "#". rewrite Len_ls; lia. }
-      iApply "Hls". iPureIntro. rewrite list_lookup_insert_ne in Hlj; try done.
+      iIntros (v j)"%Hvj %Hj". destruct (decide (j = i)) as [-> | Hij].
+      { rewrite list_lookup_insert in Hvj. inversion Hvj. subst v. done. lia. }
+      iApply "Hvs". iPureIntro. rewrite list_lookup_insert_ne in Hvj; try done.
       iPureIntro; lia.
   Qed.
 
@@ -325,19 +309,10 @@ Module IMPL1 : NODE_IMPL.
     { apply lookup_lt_is_Some_2. rewrite replicate_length. lia. }
     iIntros "!> Htl". wp_pures.
     wp_apply (createTail_rec_spec with "[Harr]").
-    { assert (replicate L #tl = (λ l : loc, #l) <$> (replicate L tl)) as ->.
-      { apply list_eq. intros i'. rewrite list_lookup_fmap. 
-        destruct (decide (i' < L)) as [Hi | Hi].
-        - rewrite !lookup_replicate_2; try done.
-        - apply not_lt in Hi. 
-          assert (L ≤ i') as H' by lia. assert (H'' := H').
-          apply (lookup_replicate_None L #tl i') in H'.
-          apply (lookup_replicate_None L tl i') in H''.
-          rewrite H' H'' /=. done. }
-      iFrame "Harr".
+    { iFrame "Harr".
       iSplit. { iPureIntro. by rewrite replicate_length. }
       iIntros (l j)"%Hlj %Hj". exfalso; lia. }
-    iIntros (ls) "(Harr & %Length_ls & Hls)".
+    iIntros (ls) "(Harr & %Length_ls & Hvs)".
     assert (∃ (m: gmap nat bool), (∀ i, i < L → m !! i = Some false) 
       ∧ dom m = gset_seq 0 (L-1)) as 
       [mark [Def_mark Dom_mark]].
@@ -354,62 +329,55 @@ Module IMPL1 : NODE_IMPL.
     iDestruct (mapsto_persist with "Htl") as ">Htl".
     iAssert (node Σ Hg1 tl L mark ∅ W) with "[- Hpost]" as "Node".
     { iExists arr, ls. iFrame "Htl Hk Harr". iSplitR. iPureIntro. 
-      split; try (done || lia). iIntros (l j)"%Hlj".
-      assert (j < L) as j_lt_L. { by rewrite -Length_ls -lookup_lt_is_Some Hlj /=. }
+      split; try (done || lia). iIntros (v j)"%Hvj".
+      assert (j < L) as j_lt_L. { by rewrite -Length_ls -lookup_lt_is_Some Hvj /=. }
       rewrite lookup_total_alt Def_mark /=; try done.
-      rewrite lookup_total_empty. iApply "Hls". iPureIntro. apply Hlj.
-      by iPureIntro. }
+      rewrite lookup_total_empty. 
+      iDestruct ("Hvs" with "[%] [%]") as "%H'". apply Hvj. done.
+      destruct v; try done. destruct v; try done. destruct l; try done. }
     iApply ("Hpost" $! tl mark). iModIntro. iFrame. iPureIntro. split; try done.
   Qed.
 
-  Lemma createHead_rec_spec Σ (Hg1 : heapGS Σ) (tl: Node) (arr: loc) (ls: list Node) 
-    (i: nat) :
-  ⊢  {{{ arr ↦∗ ((fun l => # (LitLoc l)) <$> ls)
-         ∗ ⌜length ls = L⌝
-         ∗ ∀ (l: loc) (j: nat), 
-           ⌜ls !! j = Some l⌝ -∗ ⌜j < i⌝ -∗
-             l ↦□ (#false, #tl) }}}
-           createHead_rec #i #arr #tl
-      {{{ (ls': list Node),
-          RET #();
-              arr ↦∗ ((fun l => # (LitLoc l)) <$> ls')
-            ∗ ⌜length ls' = L⌝
-            ∗ ∀ (l: loc) (j: nat), 
-              ⌜ls' !! j = Some l⌝ -∗ ⌜j < L⌝ -∗
-                l ↦□ (#false, #tl) }}}.
+  Lemma createHead_rec_spec Σ (Hg1 : heapGS Σ) (tl arr : loc) (vs: list val) (i: nat) :
+  ⊢ {{{  arr ↦∗ vs
+         ∗ ⌜length vs = L⌝
+         ∗ ∀ (v: val) (j: nat), 
+            ⌜vs !! j = Some v⌝ -∗ ⌜j < i⌝ -∗
+              (⌜match v with 
+              | InjRV #(LitLoc l) => l = tl
+              | _ => False end⌝) }}}
+          createHead_rec #i #arr #tl
+    {{{ (vs': list val),
+        RET #();
+            arr ↦∗ vs'
+          ∗ ⌜length vs' = L⌝
+          ∗ ∀ (v: val) (j: nat), 
+            ⌜vs' !! j = Some v⌝ -∗ ⌜j < L⌝ -∗
+              (⌜match v with 
+              | InjRV #(LitLoc l) => l = tl
+              | _ => False end⌝) }}}.
   Proof.
-    iIntros (Φ) "!> Hpre Hpost". iLöb as "IH" forall (i ls).
-    iDestruct "Hpre" as "(Harr & %Len_ls & Hls)".
+    iIntros (Φ) "!> Hpre Hpost". iLöb as "IH" forall (i vs).
+    iDestruct "Hpre" as "(Harr & %Len_ls & Hvs)".
     wp_lam. wp_pures. destruct (bool_decide (L ≤ i)%Z) eqn: Hi; wp_pures.
-    - iApply ("Hpost" $! ls). iFrame. iSplitR; first by iPureIntro.
-      iModIntro. iIntros (l j)"%Hlj %j_le_L".
-      rewrite bool_decide_eq_true in Hi. iApply "Hls"; try done.
+    - iApply ("Hpost" $! vs). iFrame. iSplitR; first by iPureIntro.
+      iModIntro. iIntros (v j)"%Hvj %j_le_h".
+      rewrite bool_decide_eq_true in Hi. iApply "Hvs"; try done.
       iPureIntro; lia.
-    - rewrite bool_decide_eq_false in Hi.
-      wp_apply wp_alloc; try done.
-      iIntros (l)"(Hl&_)". wp_pures. wp_bind (_ <- _)%E.
-      iApply fupd_wp. iDestruct (mapsto_persist with "Hl") as ">#Hl". iModIntro.
-      iApply (wp_store_offset _ _ arr i with "Harr").
-      { apply lookup_lt_is_Some_2. rewrite fmap_length Len_ls. lia. }
+    - rewrite bool_decide_eq_false in Hi. wp_bind (_ <- _)%E.
+      iApply (wp_store_offset _ _ arr i vs with "Harr").
+      { apply lookup_lt_is_Some_2. lia. }
       iIntros "!> Harr". wp_pures.
       assert (Z.add i 1 = (i+1)%nat) as -> by lia. 
-      iSpecialize ("IH" $! (i+1) (<[i:=l]>ls)).
-      iApply ("IH" with "[Harr Hls]"); try done.
-      assert ((λ l0 : loc, #l0) <$> <[i:=l]> ls = 
-                  <[i:=#l]> ((λ l0 : loc, #l0) <$> ls)) as ->.
-      { apply list_eq. intros i'. 
-        destruct (decide (i' = i)) as [-> | Hi'].
-        rewrite list_lookup_fmap !list_lookup_insert /=. done.
-        rewrite Len_ls; lia. rewrite fmap_length Len_ls. lia.
-        rewrite list_lookup_fmap !list_lookup_insert_ne /=; try done.
-        by rewrite list_lookup_fmap. }
+      iSpecialize ("IH" $! (i+1) (<[i:= InjRV #tl]>vs)).
+      iApply ("IH" with "[Harr Hvs]"); try done.
       iFrame "Harr". iSplitR. { iPureIntro. by rewrite insert_length. }
-      iIntros (l' j)"%Hlj %Hj". destruct (decide (j = i)) as [-> | Hij].
-      { rewrite list_lookup_insert in Hlj. inversion Hlj. subst l'.
-        iFrame "#". rewrite Len_ls; lia. }
-      iApply "Hls". iPureIntro. rewrite list_lookup_insert_ne in Hlj; try done.
+      iIntros (v j)"%Hvj %Hj". destruct (decide (j = i)) as [-> | Hij].
+      { rewrite list_lookup_insert in Hvj. inversion Hvj. done. lia. }
+      iApply "Hvs". iPureIntro. rewrite list_lookup_insert_ne in Hvj; try done.
       iPureIntro; lia.
   Qed.
+
 
   Lemma createHead_spec Σ Hg1 (tl : Node) :
   ⊢  {{{ True }}}
@@ -434,18 +402,9 @@ Module IMPL1 : NODE_IMPL.
     { apply lookup_lt_is_Some_2. rewrite replicate_length. lia. }
     iIntros "!> Hd". wp_pures.
     wp_apply (createHead_rec_spec with "[Harr]").
-    { assert (replicate L #tl = (λ l : loc, #l) <$> (replicate L tl)) as ->.
-      { apply list_eq. intros i'. rewrite list_lookup_fmap. 
-        destruct (decide (i' < L)) as [Hi | Hi].
-        - rewrite !lookup_replicate_2; try done.
-        - apply not_lt in Hi. 
-          assert (L ≤ i') as H' by lia. assert (H'' := H').
-          apply (lookup_replicate_None L #tl i') in H'.
-          apply (lookup_replicate_None L tl i') in H''.
-          rewrite H' H'' /=. done. }
-      iFrame "Harr". iSplit. { iPureIntro. by rewrite replicate_length. }
-      iIntros (l j)"%Hlj %Hj". exfalso; lia. }
-    iIntros (ls) "(Harr & %Length_ls & Hls)".
+    { iFrame "Harr". iSplit. { iPureIntro. by rewrite replicate_length. }
+      iIntros (v j)"%Hvj %Hj". exfalso; lia. }
+    iIntros (vs) "(Harr & %Length_vs & Hvs)".
     assert (∃ (m: gmap nat bool), (∀ i, i < L → m !! i = Some false) 
       ∧ dom m = gset_seq 0 (L-1)) as 
       [mark [Def_mark Dom_mark]].
@@ -469,70 +428,65 @@ Module IMPL1 : NODE_IMPL.
     iDestruct (mapsto_persist with "Hk") as ">Hk".
     iDestruct (mapsto_persist with "Hd") as ">Hd".
     iAssert (node Σ Hg1 hd L mark next 0) with "[- Hpost]" as "Node".
-    { iExists arr, ls. iFrame "Hd Hk Harr". iSplitR. iPureIntro.  
-      split; try (done || lia). iIntros (l j)"%Hlj".
-      assert (j < L) as j_lt_L. { by rewrite -Length_ls -lookup_lt_is_Some Hlj /=. }
+    { iExists arr, vs. iFrame "Hd Hk Harr". iSplitR. iPureIntro.  
+      split; try (done || lia). iIntros (v j)"%Hvj".
+      assert (j < L) as j_lt_L. { by rewrite -Length_vs -lookup_lt_is_Some Hvj /=. }
       rewrite lookup_total_alt Def_mark /=; try done.
       rewrite lookup_total_alt Def_next /=; try done.
-      iApply "Hls". iPureIntro. apply Hlj. by iPureIntro. }
+      iDestruct ("Hvs" with "[%] [%]") as "%H'". apply Hvj. done.
+      destruct v; try done. destruct v; try done. destruct l; try done. }
     iApply ("Hpost" $! hd mark next). iModIntro. iFrame. iPureIntro. split; try done.
   Qed.
 
-  Lemma createNode_rec_spec Σ (Hg1 : heapGS Σ) (arr succs: loc) (ls ss: list Node) (h i: nat) :
-  ⊢  {{{ is_array Σ Hg1 succs ss 
-         ∗ arr ↦∗ ((fun l => # (LitLoc l)) <$> ls)
-         ∗ ⌜length ls = h⌝
+    
+  Lemma createNode_rec_spec Σ (Hg1 : heapGS Σ) (arr succs: loc) (vs: list val) 
+    (ss: list Node) (h i: nat) :
+  ⊢ {{{ is_array Σ Hg1 succs ss 
+         ∗ arr ↦∗ vs
+         ∗ ⌜length vs = h⌝
          ∗ ⌜h <= length ss⌝
-         ∗ ∀ (l: loc) (j: nat), 
-           ⌜ls !! j = Some l⌝ -∗ ⌜j < i⌝ -∗
-             l ↦□ (#false, #((ss !!! j): Node)) }}}
-           createNode_rec #i #h #arr #succs
-      {{{ (ls': list Node),
-          RET #();
-              is_array Σ Hg1 succs ss
-            ∗ arr ↦∗ ((fun l => # (LitLoc l)) <$> ls')
-            ∗ ⌜length ls' = h⌝
-            ∗ ∀ (l: loc) (j: nat), 
-              ⌜ls' !! j = Some l⌝ -∗ ⌜j < h⌝ -∗
-                l ↦□ (#false, #((ss !!! j): Node)) }}}.
+         ∗ ∀ (v: val) (j: nat), 
+            ⌜vs !! j = Some v⌝ -∗ ⌜j < i⌝ -∗
+              (⌜match v with 
+              | InjRV #(LitLoc l) => ss !!! j = l
+              | _ => False end⌝) }}}
+          createNode_rec #i #h #arr #succs
+    {{{ (vs': list val),
+        RET #();
+            is_array Σ Hg1 succs ss
+          ∗ arr ↦∗ vs'
+          ∗ ⌜length vs' = h⌝
+          ∗ ∀ (v: val) (j: nat), 
+            ⌜vs' !! j = Some v⌝ -∗ ⌜j < h⌝ -∗
+              (⌜match v with 
+              | InjRV #(LitLoc l) => ss !!! j = l
+              | _ => False end⌝) }}}.
   Proof.
-    iIntros (Φ) "!> Hpre Hpost". iLöb as "IH" forall (i ls).
-    iDestruct "Hpre" as "(Hsuccs & Harr & %Len_ls & %Hss & Hls)".
+    iIntros (Φ) "!> Hpre Hpost". iLöb as "IH" forall (i vs).
+    iDestruct "Hpre" as "(Hsuccs & Harr & %Len_ls & %Hss & Hvs)".
     wp_lam. wp_pures. destruct (bool_decide (h ≤ i)%Z) eqn: Hi; wp_pures.
-    - iApply ("Hpost" $! ls). iFrame. iSplitR; first by iPureIntro.
-      iModIntro. iIntros (l j)"%Hlj %j_le_h".
-      rewrite bool_decide_eq_true in Hi. iApply "Hls"; try done.
+    - iApply ("Hpost" $! vs). iFrame. iSplitR; first by iPureIntro.
+      iModIntro. iIntros (v j)"%Hvj %j_le_h".
+      rewrite bool_decide_eq_true in Hi. iApply "Hvs"; try done.
       iPureIntro; lia.
     - rewrite bool_decide_eq_false in Hi. 
       assert (∃ si, ss !! i = Some si) as [si Def_si].
       { apply lookup_lt_is_Some. lia. }  
       wp_apply (wp_load_offset _ _ _ _ _ _ #si with "[Hsuccs]"); try done.
       { by rewrite list_lookup_fmap Def_si /=. }
-      iIntros "Hsuccs". wp_pures. wp_apply wp_alloc; try done.
-      iIntros (l)"(Hl&_)". wp_pures. wp_bind (_ <- _)%E.
-      iApply fupd_wp.
-      iDestruct (mapsto_persist with "Hl") as ">Hl".
-      iModIntro.
-      iApply (wp_store_offset _ _ arr i with "Harr").
-      { apply lookup_lt_is_Some_2. rewrite fmap_length Len_ls. lia. }
+      iIntros "Hsuccs". wp_pures. wp_bind (_ <- _)%E.
+      iApply (wp_store_offset _ _ arr i vs with "Harr").
+      { apply lookup_lt_is_Some_2. lia. }
       iIntros "!> Harr". wp_pures.
       assert (Z.add i 1 = (i+1)%nat) as -> by lia. 
-      iSpecialize ("IH" $! (i+1) (<[i:=l]>ls)).
-      iApply ("IH" with "[Hsuccs Harr Hl Hls]"); try done.
-      assert ((λ l0 : loc, #l0) <$> <[i:=l]> ls = 
-                  <[i:=#l]> ((λ l0 : loc, #l0) <$> ls)) as ->.
-      { apply list_eq. intros i'. 
-        destruct (decide (i' = i)) as [-> | Hi'].
-        rewrite list_lookup_fmap !list_lookup_insert /=. done.
-        rewrite Len_ls; lia. rewrite fmap_length Len_ls. lia.
-        rewrite list_lookup_fmap !list_lookup_insert_ne /=; try done.
-        by rewrite list_lookup_fmap. }
+      iSpecialize ("IH" $! (i+1) (<[i:= InjRV #si]>vs)).
+      iApply ("IH" with "[Hsuccs Harr Hvs]"); try done.
       iFrame "Hsuccs Harr". iSplitR. { iPureIntro. by rewrite insert_length. }
       iSplitR. by iPureIntro.
-      iIntros (l' j)"%Hlj %Hj". destruct (decide (j = i)) as [-> | Hij].
-      { rewrite list_lookup_insert in Hlj. inversion Hlj. subst l'.
-        rewrite list_lookup_total_alt Def_si /=. iFrame. rewrite Len_ls; lia. }
-      iApply "Hls". iPureIntro. rewrite list_lookup_insert_ne in Hlj; try done.
+      iIntros (v j)"%Hvj %Hj". destruct (decide (j = i)) as [-> | Hij].
+      { rewrite list_lookup_insert in Hvj. inversion Hvj. subst v.
+        rewrite list_lookup_total_alt Def_si /=. done. lia. }
+      iApply "Hvs". iPureIntro. rewrite list_lookup_insert_ne in Hvj; try done.
       iPureIntro; lia.
   Qed.
 
@@ -562,20 +516,11 @@ Module IMPL1 : NODE_IMPL.
     { apply lookup_lt_is_Some_2. rewrite replicate_length. lia. }
     iIntros "!> Hn". wp_pures.
     wp_apply (createNode_rec_spec _ _ _ _ _ _ h _ with "[Hsuccs Harr]").
-    { assert (replicate h #n = (λ l : loc, #l) <$> (replicate h n)) as ->.
-      { apply list_eq. intros i'. rewrite list_lookup_fmap. 
-        destruct (decide (i' < h)) as [Hi | Hi].
-        - rewrite !lookup_replicate_2; try done.
-        - apply not_lt in Hi. 
-          assert (h ≤ i') as H' by lia. assert (H'' := H').
-          apply (lookup_replicate_None h #n i') in H'.
-          apply (lookup_replicate_None h n i') in H''.
-          rewrite H' H'' /=. done. }
-      iFrame "Hsuccs Harr".
+    { iFrame "Hsuccs Harr".
       iSplit. { iPureIntro. by rewrite replicate_length. }
       iSplitR. iPureIntro; lia.
       iIntros (l j)"%Hlj %Hj". exfalso; lia. }
-    iIntros (ls) "(Hsuccs & Harr & %Length_ls & Hls)".
+    iIntros (vs) "(Hsuccs & Harr & %Length_vs & #Hvs)".
     assert (∃ (m: gmap nat bool), (∀ i, i < h → m !! i = Some false) 
       ∧ dom m = gset_seq 0 (h-1)) as 
       [mark [Def_mark Dom_mark]].
@@ -586,8 +531,8 @@ Module IMPL1 : NODE_IMPL.
     { apply next_map. lia. }
     wp_pures. iApply ("Hpost" $! n h mark next).
     iFrame "Hsuccs". iSplitL; last first.
-    { iPureIntro. repeat split; try (done || lia). }  
-    iExists arr, ls.
+    { iPureIntro; try done. }  
+    iExists arr, vs.
     assert (<[1:=#arr]> (replicate 2 (#k, #h)%V) = (#k, #h)%V :: #arr :: []) as ->.
     { rewrite /replicate /=. done. }
     iAssert (n ↦ (#k, #h)%V ∗ (n +ₗ 1) ↦ #arr)%I with "[Hn]" as "(Hk & Hn)".
@@ -597,12 +542,14 @@ Module IMPL1 : NODE_IMPL.
         lia. destruct n; try done. } iFrame. }
     iDestruct (mapsto_persist with "Hk") as ">Hk".
     iDestruct (mapsto_persist with "Hn") as ">Hn".
-    iFrame "Hn Hk Harr". iSplitR. iPureIntro. split; try (done || lia).
-    iModIntro. iIntros (l j)"%Hlj".
-    assert (j < h) as j_lt_h. { by rewrite -Length_ls -lookup_lt_is_Some Hlj /=. }
-    rewrite lookup_total_alt Def_mark /=; try done.
-    rewrite lookup_total_alt Def_next /=; try done. iSpecialize ("Hls" $! l j).
-    iDestruct ("Hls" with "[%] [%]") as "H'"; try done.
+    iFrame "Hn Hk Harr". iSplitR. iPureIntro. split. done. lia. 
+    iModIntro. iIntros (v j)"%Hvj".
+    assert (j < h) as j_lt_h. { by rewrite -Length_vs -lookup_lt_is_Some Hvj /=. }
+    iSpecialize ("Hvs" $! v j). iDestruct ("Hvs" with "[%] [%]") as "H'"; try done.
+    destruct v; try done. destruct v; try done. destruct l; try done.
+    iDestruct "H'" as %Hssj. iPureIntro.
+    rewrite !lookup_total_alt Def_mark /=; try done. 
+    rewrite Def_next; try done. 
   Qed.
 
   Lemma getHeight_spec Σ Hg1 (n: Node) :
@@ -613,10 +560,10 @@ Module IMPL1 : NODE_IMPL.
     iIntros (Φ) "AU".
     wp_lam. wp_pures. wp_bind (! _)%E.
     iMod "AU" as (h0 m0 nx0 k0) "[Node [_ Hclose]]".
-    iDestruct "Node" as (arr0 ls0) "(#Hk0 & #Hn0 & Harr & %Len_vs0 & #Hls0)".
+    iDestruct "Node" as (arr0 vs0) "(#Hk0 & #Hn0 & Harr & %Len_vs0 & #Hvs0)".
     wp_load. 
     iMod ("Hclose" with "[Harr]") as "AU".
-    { iFrame "%". iExists arr0, ls0. iFrame "∗#%". }
+    { iFrame "%". iExists arr0, vs0. iFrame "∗#%". }
     iModIntro. wp_pures. done.
   Qed.
 
@@ -635,6 +582,7 @@ Module IMPL1 : NODE_IMPL.
     iModIntro. wp_pures. done.
   Qed.
 
+
   Lemma findNext_spec Σ Hg1 (n: Node) (i: nat) :
     ⊢ <<{ ∀∀ h mark next k, node Σ Hg1 n h mark next k ∗ ⌜i < h⌝ }>>
           findNext #n #i @ ∅
@@ -645,26 +593,27 @@ Module IMPL1 : NODE_IMPL.
     iIntros (Φ) "AU".
     wp_lam. wp_pures. wp_bind (! _)%E.
     iMod "AU" as (h0 m0 nx0 k0) "[(Node&%Hi0) [Hclose _]]".
-    iDestruct "Node" as (arr0 ls0) "(#Hk0 & #Hn0 & Harr & %Len_vs0 & #Hls0)".
+    iDestruct "Node" as (arr0 vs0) "(#Hk0 & #Hn0 & Harr & %Len_vs0 & #Hvs0)".
     wp_load. 
     iMod ("Hclose" with "[Harr]") as "AU".
-    { iFrame "%". iExists arr0, ls0. iFrame "∗#%". }
+    { iFrame "%". iExists arr0, vs0. iFrame "∗#%". }
     iModIntro. wp_pures. wp_bind (! _)%E.
     iMod "AU" as (h1 m1 nx1 k1) "[(Node&%Hi1) [_ Hclose]]".
-    iDestruct "Node" as (arr1 ls1) "(#Hk1 & #Hn1 & Harr & %Len_vs1 & #Hls1)".
+    iDestruct "Node" as (arr1 vs1) "(#Hk1 & #Hn1 & Harr & %Len_vs1 & #Hvs1)".
     iDestruct (mapsto_agree with "[$Hn0] [$Hn1]") as "%H'". 
     inversion H'; subst arr1; clear H'.
-    assert (∃ li, ls1 !! i = Some li) as [li Def_li].
-    { apply lookup_lt_is_Some. destruct Len_vs1 as [-> _]. done.  }  
+    assert (∃ vi, vs1 !! i = Some vi) as [vi Def_vi].
+    { apply lookup_lt_is_Some. destruct Len_vs1 as [-> _]. done. }  
     wp_apply (wp_load_offset _ _ _ (DfracOwn (pos_to_Qp 1)) _ 
-        _ #li with "[Harr]"); try done.
-    { by rewrite list_lookup_fmap Def_li /=. }
+        _ vi with "[Harr]"); try done.
     iIntros "Harr".
-    iDestruct ("Hls1" with "[%]") as "H'". apply Def_li.
+    iDestruct ("Hvs1" with "[%]") as "H'". apply Def_vi.
     iSpecialize ("Hclose" $! (m1 !!! i) (nx1 !!! i)).
     iMod ("Hclose" with "[Harr]") as "HΦ".
-    { iSplitL. iExists arr0, ls1. iFrame "∗#%". by iPureIntro. }
-    iModIntro. wp_pures. wp_load. by wp_pures.
+    { iSplitL. iExists arr0, vs1. iFrame "∗#%". by iPureIntro. }
+    iModIntro. wp_pures. destruct vi; try done; destruct vi; try done; 
+    destruct l; try done; wp_pures.
+    all: iDestruct "H'" as %[H' H'']; rewrite H' H''; done.
   Qed.
   
   Lemma markNode_spec Σ Hg1 (n: Node) (i: nat) :
@@ -682,88 +631,73 @@ Module IMPL1 : NODE_IMPL.
     iIntros (Φ) "AU". iLöb as "IH".
     wp_lam. wp_pures. wp_bind (! _)%E.
     iMod "AU" as (h0 m0 nx0 k0) "[(Node&%Hi0) [Hclose _]]".
-    iDestruct "Node" as (arr0 ls0) "(#Hk0 & #Hn0 & Harr & %Len_vs0 & #Hls0)".
+    iDestruct "Node" as (arr0 vs0) "(#Hk0 & #Hn0 & Harr & %Len_vs0 & #Hvs0)".
     wp_load. 
     iMod ("Hclose" with "[Harr]") as "AU".
-    { iFrame "%". iExists arr0, ls0. iFrame "∗#%". }
+    { iFrame "%". iExists arr0, vs0. iFrame "∗#%". }
     iModIntro. wp_pures. wp_bind (! _)%E.
     iMod "AU" as (h1 m1 nx1 k1) "[(Node&%Hi1) HAU]".
-    iDestruct "Node" as (arr1 ls1) "(#Hk1 & #Hn1 & Harr & %Len_vs1 & #Hls1)".
+    iDestruct "Node" as (arr1 vs1) "(#Hk1 & #Hn1 & Harr & %Len_vs1 & #Hvs1)".
     iDestruct (mapsto_agree with "[$Hn0] [$Hn1]") as "%H'". 
     inversion H'; subst arr1; clear H'.
-    assert (∃ li, ls1 !! i = Some li) as [li Def_li].
+    assert (∃ vi, vs1 !! i = Some vi) as [vi Def_vi].
     { apply lookup_lt_is_Some. by destruct Len_vs1 as [-> _]. }  
     wp_apply (wp_load_offset _ _ _ (DfracOwn (pos_to_Qp 1)) _ 
-        _ #li with "[Harr]"); try done.
-    { by rewrite list_lookup_fmap Def_li /=. }
+        _ vi with "[Harr]"); try done.
     iIntros "Harr".
-    iDestruct ("Hls1" with "[%]") as "H'". apply Def_li.
+    iDestruct ("Hvs1" with "[%]") as "H'". apply Def_vi.
     destruct (decide (m1 !!! i = true)) as [Hmi | Hmi].
     - iDestruct "HAU" as "[_ Hclose]".
       iSpecialize ("Hclose" $! false m1).
       iMod ("Hclose" with "[Harr]") as "HΦ".
-      { iSplitL. iExists arr0, ls1. iFrame "∗#%".
+      { iSplitL. iExists arr0, vs1. iFrame "∗#%".
         by iPureIntro. }
-      iModIntro. wp_pures. wp_load. wp_pures.
-      rewrite Hmi. wp_pures. done.
-    - apply not_true_is_false in Hmi.
+      iModIntro. wp_pures. rewrite Hmi. 
+      destruct vi; try done; destruct vi; try done; destruct l; try done; last first.
+      { iDestruct "H'" as %[? _]. done. } wp_pures. done.
+    - apply not_true_is_false in Hmi. rewrite Hmi.
+      destruct vi; try done; destruct vi; try done; destruct l; try done.
+      { iDestruct "H'" as %[? _]. done. }
       iDestruct "HAU" as "[Hclose _]".
       iMod ("Hclose" with "[Harr]") as "AU".
-      { iFrame "%". iExists arr0, ls1. iFrame "∗#%". }
-      iModIntro. wp_pures. wp_load. wp_pures.
-      rewrite Hmi. wp_pures.
-      wp_alloc li_new as "Hnew". wp_pures.
+      { iFrame "%". iExists arr0, vs1. iFrame "∗#%". }
+      iModIntro. wp_pures.
       wp_bind (CmpXchg _ _ _)%E.
       iMod "AU" as (h2 m2 nx2 k2) "[(Node&%Hi2) HAU]".
-      iDestruct "Node" as (arr2 ls2) "(#Hk2 & #Hn2 & Harr & %Len_vs2 & #Hls2)".
+      iDestruct "Node" as (arr2 vs2) "(#Hk2 & #Hn2 & Harr & %Len_vs2 & #Hvs2)".
       iDestruct (mapsto_agree with "[$Hn0] [$Hn2]") as "%H'". 
       inversion H'; subst arr2; clear H'.
-      assert (∃ li', ls2 !! i = Some li') as [li' Def_li'].
-      { apply lookup_lt_is_Some. by destruct Len_vs2 as [-> _].  }
-      destruct (decide (li' = li)) as [-> | Des_li].
+      assert (∃ vi', vs2 !! i = Some vi') as [vi' Def_vi'].
+      { apply lookup_lt_is_Some. by destruct Len_vs2 as [-> _]. }
+      destruct (decide (vi' = InjRV #l)) as [-> | Des_vi].
       + wp_apply (wp_cmpxchg_suc_offset _ _ _ _ _ _ with "[Harr]"); 
           try done.
-        { by rewrite list_lookup_fmap Def_li' /=. }
         { left; try done. }
         iIntros "Harr".
         iDestruct "HAU" as "[_ Hclose]".
         iSpecialize ("Hclose" $! true (<[i:=true]> m2)).
-        iDestruct (mapsto_persist with "Hnew") as ">#Hnew'".
-        iDestruct ("Hls2" with "[%]") as "H''". apply Def_li'.
-        iDestruct (mapsto_agree with "H' H''") as "%H'". inversion H'.
+        iDestruct ("Hvs2" with "[%]") as "H''". apply Def_vi'.
+        iEval (simpl) in "H''". 
         iMod ("Hclose" with "[Harr]") as "HΦ".
-        { iSplitL. iExists arr0, (<[i:= li_new]> ls2). iFrame "#".
-          iSplitL "Harr". 
-          assert (((λ l : loc, #l) <$> <[i:=li_new]> ls2) = 
-            <[i:=#li_new]> ((λ l : loc, #l) <$> ls2)) as ->.
-          { destruct Len_vs2 as [Len_vs2 _]. apply list_eq. intros i'. 
-            destruct (decide (i' = i)) as [-> | Hi'].
-            rewrite list_lookup_fmap !list_lookup_insert /=. done.
-            by rewrite fmap_length Len_vs2. by rewrite Len_vs2. 
-            rewrite list_lookup_fmap !list_lookup_insert_ne /=; try done.
-            by rewrite list_lookup_fmap. }
-          iFrame "Harr". iSplitR. { iPureIntro. by rewrite insert_length. }
-          iIntros (l j)"%Hlj". destruct (decide (j = i)) as [-> | Hj].
+        { iDestruct "H''" as %[? ?]. iSplitL; last by iPureIntro. 
+          iExists arr0, (<[i:= InjLV #l]> vs2). iFrame "# Harr".
+          iSplitR. { iPureIntro. by rewrite insert_length. }
+          iIntros (v j)"%Hvj". destruct (decide (j = i)) as [-> | Hj].
+          rewrite list_lookup_insert in Hvj; last by lia. inversion Hvj.
           assert (<[i:=true]> m2 !!! i = true) as ->.
-          by rewrite lookup_total_insert.
-          rewrite list_lookup_insert in Hlj. inversion Hlj.
-          rewrite H1; try done. by destruct Len_vs2 as [-> _].
-          assert (<[i:=true]> m2 !!! j = m2 !!! j) as ->.
-          by rewrite lookup_total_insert_ne.
-          rewrite list_lookup_insert_ne in Hlj; try done.
-          iClear "H' H''".
-          iDestruct ("Hls2" with "[%]") as "H'". apply Hlj.
-          done.
-          by iPureIntro. }
+          by rewrite lookup_total_insert. by iPureIntro.
+          rewrite list_lookup_insert_ne in Hvj; try done. iClear "H'".
+          iDestruct ("Hvs2" with "[%]") as "H'". apply Hvj.
+          destruct v; try done; destruct v; try done; destruct l1; try done.
+          all: iDestruct "H'" as %[? ?]. 
+          all: iPureIntro; rewrite lookup_total_insert_ne; try done. }
         iModIntro. wp_pures. done.
-      + wp_apply (wp_cmpxchg_fail_offset _ _ _ _ _ _ #li' with "[Harr]"); 
+      + wp_apply (wp_cmpxchg_fail_offset _ _ _ _ _ _ vi' with "[Harr]"); 
           try done.
-        { by rewrite list_lookup_fmap Def_li' /=. }
-        { by intros [=->]. }
-        { left; try done. }
+        { right; try done. }
         iIntros "Harr". iDestruct "HAU" as "[Hclose _]".
         iMod ("Hclose" with "[Harr]") as "AU".
-        { iSplitL; last by iPureIntro. iExists arr0, ls2. iFrame "∗#%". }
+        { iSplitL; last by iPureIntro. iExists arr0, vs2. iFrame "∗#%". }
         iModIntro. wp_pures. by iApply "IH".
   Qed.  
 
@@ -788,87 +722,82 @@ Module IMPL1 : NODE_IMPL.
     iIntros "Hproph" (Φ) "AU". iLöb as "IH" forall (pvs).
     wp_lam. wp_pures. wp_bind (! _)%E.
     iMod "AU" as (h0 m0 nx0 k0) "[(Node&%Hi0) [Hclose _]]".
-    iDestruct "Node" as (arr0 ls0) "(#Hk0 & #Hn0 & Harr & %Len_vs0 & #Hls0)".
+    iDestruct "Node" as (arr0 vs0) "(#Hk0 & #Hn0 & Harr & %Len_vs0 & #Hvs0)".
     wp_load. 
     iMod ("Hclose" with "[Harr]") as "AU".
-    { iFrame "∗%". iExists arr0, ls0. iFrame "∗#%". }
+    { iFrame "%". iExists arr0, vs0. iFrame "∗#%". }
     iModIntro. wp_pures. wp_bind (! _)%E.
     iMod "AU" as (h1 m1 nx1 k1) "[(Node&%Hi1) HAU]".
-    iDestruct "Node" as (arr1 ls1) "(#Hk1 & #Hn1 & Harr & %Len_vs1 & #Hls1)".
+    iDestruct "Node" as (arr1 vs1) "(#Hk1 & #Hn1 & Harr & %Len_vs1 & #Hvs1)".
     iDestruct (mapsto_agree with "[$Hn0] [$Hn1]") as "%H'". 
     inversion H'; subst arr1; clear H'.
-    assert (∃ li, ls1 !! 0 = Some li) as [li Def_li].
+    assert (∃ vi, vs1 !! 0 = Some vi) as [vi Def_vi].
     { apply lookup_lt_is_Some. by destruct Len_vs1 as [-> _]. }  
     wp_apply (wp_load_offset _ _ _ (DfracOwn (pos_to_Qp 1)) _ 
-        _ #li with "[Harr]"); try done.
-    { by rewrite list_lookup_fmap Def_li /=. }
+        _ vi with "[Harr]"); try done.
     iIntros "Harr".
-    iDestruct ("Hls1" with "[%]") as "H'". apply Def_li.
+    iDestruct ("Hvs1" with "[%]") as "H'". apply Def_vi.
     destruct (decide (m1 !!! 0 = true)) as [Hmi | Hmi].
     - iDestruct "HAU" as "[_ Hclose]".
       iSpecialize ("Hclose" $! false m1).
       iMod ("Hclose" with "[Harr Hproph]") as "HΦ".
-      { iFrame. iSplitL. iExists arr0, ls1. iFrame "∗#%". by iPureIntro. }
-      iModIntro. wp_pures. wp_load. wp_pures.
-      rewrite Hmi. wp_pures. done.
-    - apply not_true_is_false in Hmi.
+      { iFrame. iSplitL. iExists arr0, vs1. iFrame "∗#%". by iPureIntro. }
+      iModIntro. wp_pures. rewrite Hmi. 
+      destruct vi; try done; destruct vi; try done; destruct l; try done; last first.
+      { iDestruct "H'" as %[? _]. done. } wp_pures. done.
+    - apply not_true_is_false in Hmi. rewrite Hmi.
+      destruct vi; try done; destruct vi; try done; destruct l; try done.
+      { iDestruct "H'" as %[? _]. done. }
       iDestruct "HAU" as "[Hclose _]".
       iMod ("Hclose" with "[Harr]") as "AU".
-      { iFrame "∗%". iExists arr0, ls1. iFrame "∗#%". }
-      iModIntro. wp_pures. wp_load. wp_pures.
-      rewrite Hmi. wp_pures.
-      wp_alloc li_new as "Hnew". wp_pures.
+      { iFrame "%". iExists arr0, vs1. iFrame "∗#%". }
+      iClear "Hvs0 Hvs1". iModIntro. wp_pures. 
       wp_bind (Resolve _ _ _)%E. 
       iMod "AU" as (h2 m2 nx2 k2) "[(Node&%Hi2) HAU]".
-      iDestruct "Node" as (arr2 ls2) "(#Hk2 & #Hn2 & Harr & %Len_vs2 & #Hls2)".
+      iDestruct "Node" as (arr2 vs2) "(#Hk2 & #Hn2 & Harr & %Len_vs2 & #Hvs2)".
       iDestruct (mapsto_agree with "[$Hn0] [$Hn2]") as "%H'". 
       inversion H'; subst arr2; clear H'.
-      destruct ls2 as [|li' ls2'] eqn: Def_ls2. 
-      { rewrite /= in Len_vs2. exfalso; lia. }
-      assert (ls2 !! 0 = Some li') as Def_li'.
-      { by rewrite Def_ls2 /=. }
-      assert (((λ l : loc, #l) <$> li' :: ls2') = 
-        #li' :: ((λ l : loc, #l) <$> ls2')) as ->.
-      { by rewrite fmap_cons. } rewrite array_cons. 
+      destruct vs2 as [|vi' vs2'] eqn: Def_vs2.
+      { clear -Len_vs2. exfalso. rewrite /= in Len_vs2. lia. } rewrite -Def_vs2.
+      assert (vs2 !! 0 = Some vi') as Def_vi'. { rewrite Def_vs2 /=. done. }
+      iEval (rewrite Def_vs2 array_cons) in "Harr". 
       iDestruct "Harr" as "(Harr0 & Harr)".
       assert (arr0 +ₗ 0%nat = arr0) as ->. { by rewrite Loc.add_0. }
-      destruct (decide (li' = li)) as [-> | Des_li].
+      destruct (decide (vi' = InjRV #l)) as [-> | Des_vi].
       + wp_apply (wp_resolve_cmpxchg_suc with "[$Harr0 $Hproph]").
         { by left. }
         iIntros "H''". iDestruct "H''" as (pvs')"(%Hpvs' & Hproph & Harr0)".
         iDestruct "HAU" as "[_ Hclose]".
         iSpecialize ("Hclose" $! true (<[0:=true]> m2)).
-        iDestruct (mapsto_persist with "Hnew") as ">#Hnew'".
-        iDestruct ("Hls2" with "[%]") as "H''". rewrite -Def_ls2. apply Def_li'.
-        iDestruct (mapsto_agree with "H' H''") as "%H'". inversion H'.
+        iDestruct ("Hvs2" with "[%]") as "H''". apply Def_vi'.
+        iEval (simpl) in "H''". 
         iMod ("Hclose" with "[Harr Harr0 Hproph]") as "HΦ".
-        { iFrame "Hproph". iSplitL. iExists arr0, (<[0:= li_new]> ls2). iFrame "#".
-          iSplitL. assert (((λ l : loc, #l) <$> <[0:=li_new]> ls2) = 
-            #li_new :: ((λ l : loc, #l) <$> ls2')) as ->.
-          { rewrite Def_ls2 /=. apply f_equal. done. } 
-          rewrite array_cons. iFrame. 
-          iSplitR. { iPureIntro. by rewrite insert_length Def_ls2. }
-          iIntros (l j)"%Hlj". destruct (decide (j = 0)) as [-> | Hj].
+        { iDestruct "H''" as %[? ?]. iFrame "Hproph". iSplitL. 
+          iExists arr0, (<[0:= InjLV #l]> vs2). iFrame "#".
+          assert (<[0:=InjLV #l]> vs2 = InjLV #l :: vs2') as H'.
+          { rewrite Def_vs2 /=. done. } rewrite H'. iFrame.
+          iSplitR. { iPureIntro. rewrite /=. rewrite /= in Len_vs2. done. }
+          iIntros (v j)"%Hvj". destruct (decide (j = 0)) as [-> | Hj].
+          rewrite /= in Hvj. inversion Hvj.
           assert (<[0:=true]> m2 !!! 0 = true) as ->.
-          by rewrite lookup_total_insert.
-          rewrite list_lookup_insert in Hlj. inversion Hlj.
-          rewrite H1; try done. destruct Len_vs2 as [Len_vs2 _]. 
-          by rewrite Def_ls2 Len_vs2.
-          assert (<[0:=true]> m2 !!! j = m2 !!! j) as ->.
-          by rewrite lookup_total_insert_ne.
-          rewrite list_lookup_insert_ne in Hlj; try done.
-          iClear "H' H''".
-          iDestruct ("Hls2" with "[%]") as "H'". rewrite -Def_ls2. apply Hlj.
-          iFrame "#". iPureIntro. repeat split; try done.
-          exists #li. rewrite Hpvs'. clear; set_solver. }
+          by rewrite lookup_total_insert. by iPureIntro.
+          rewrite -H' in Hvj. rewrite list_lookup_insert_ne in Hvj; try done. 
+          iClear "H'".
+          iDestruct ("Hvs2" with "[%]") as "H'". apply Hvj.
+          destruct v; try done; destruct v; try done; destruct l1; try done.
+          all: iDestruct "H'" as %[? ?]; iPureIntro. 
+          all: try (rewrite lookup_total_insert_ne; try done).
+          repeat split; try done. exists (InjRV #l). rewrite Hpvs'. clear; set_solver. }
         iModIntro. wp_pures. done.
       + wp_apply (wp_resolve_cmpxchg_fail with "[$Harr0 $Hproph]").
         { by intros [=->]. }
-        { by left. }
+        { by right. }
         iIntros "H''". iDestruct "H''" as (pvs')"(%Hpvs' & Hproph & Harr0)".
         iDestruct "HAU" as "[Hclose _]".
         iMod ("Hclose" with "[Harr Harr0]") as "AU".
-        { iSplitL; last by iPureIntro. iExists arr0, (li' :: ls2'). iFrame "∗#%". }
+        { iSplitL; last by iPureIntro. iExists arr0, (vi' :: vs2').
+          rewrite -Def_vs2. iFrame "∗#%". rewrite Def_vs2 array_cons. iFrame.
+          by iPureIntro. }
         iModIntro. wp_pures. iApply ("IH" with "[$Hproph] [AU]"); try done.
         iAuIntro. rewrite /atomic_acc /=. iClear "#". 
         iMod "AU" as (h3 m3 nx3 k3)"[H' H'']". iModIntro.
@@ -876,10 +805,10 @@ Module IMPL1 : NODE_IMPL.
         * iDestruct "H''" as "[H'' _]". iApply "H''".
         * iDestruct "H''" as "[_ H'']". iIntros (res m3' prf pvs'').
           iIntros "(Node & Hproph & %Hprf & Hres)". 
-          iSpecialize ("H''" $! res m3' (((#li', #false)%V, #()) :: prf) pvs'').
+          iSpecialize ("H''" $! res m3' (((vi', #false)%V, #()) :: prf) pvs'').
           iMod ("H''" with "[Node Hproph Hres]") as "HΦ".
           iFrame "Node Hproph". iSplitR. iPureIntro. 
-          rewrite Forall_cons; split; try done. by exists #li'.
+          rewrite Forall_cons; split; try done. by exists vi'.
           destruct res; iDestruct "Hres" as "%H'"; iPureIntro; 
             repeat split; try apply H'. destruct H' as (_&_&[v1 Def_pvs']).
           rewrite Def_pvs' in Hpvs'. exists v1. rewrite Hpvs'. done.
@@ -905,98 +834,83 @@ Module IMPL1 : NODE_IMPL.
     iIntros (Φ) "AU". iLöb as "IH".
     wp_lam. wp_pures. wp_bind (! _)%E.
     iMod "AU" as (h0 m0 nx0 k0) "[(Node&%Hi0) [Hclose _]]".
-    iDestruct "Node" as (arr0 ls0) "(#Hk0 & #Hn0 & Harr & %Len_vs0 & #Hls0)".
+    iDestruct "Node" as (arr0 vs0) "(#Hk0 & #Hn0 & Harr & %Len_vs0 & #Hvs0)".
     wp_load. 
     iMod ("Hclose" with "[Harr]") as "AU".
-    { iSplitL; last by iPureIntro. iExists arr0, ls0. iFrame "∗#%". }
+    { iSplitL; last by iPureIntro. iExists arr0, vs0. iFrame "∗#%". }
     iModIntro. wp_pures. wp_bind (! _)%E.
     iMod "AU" as (h1 m1 nx1 k1) "[(Node&%Hi1) HAU]".
-    iDestruct "Node" as (arr1 ls1) "(#Hk1 & #Hn1 & Harr & %Len_vs1 & #Hls1)".
+    iDestruct "Node" as (arr1 vs1) "(#Hk1 & #Hn1 & Harr & %Len_vs1 & #Hvs1)".
     iDestruct (mapsto_agree with "[$Hn0] [$Hn1]") as "%H'". 
     inversion H'; subst arr1; clear H'.
-    assert (∃ li, ls1 !! i = Some li) as [li Def_li].
+    assert (∃ vi, vs1 !! i = Some vi) as [vi Def_vi].
     { apply lookup_lt_is_Some. by destruct Len_vs1 as [-> _]. }  
     wp_apply (wp_load_offset _ _ _ (DfracOwn (pos_to_Qp 1)) _ 
-        _ #li with "[Harr]"); try done.
-    { by rewrite list_lookup_fmap Def_li /=. }
+        _ vi with "[Harr]"); try done.
     iIntros "Harr".
-    iDestruct ("Hls1" with "[%]") as "H'". apply Def_li.
-    destruct (decide (m1 !!! i = true)) as [Hmi | Hmi].
+    iDestruct ("Hvs1" with "[%]") as "H'". apply Def_vi.
+    destruct vi; try done.
     - iDestruct "HAU" as "[_ Hclose]".
       iSpecialize ("Hclose" $! false nx1).
+      destruct vi; try done. destruct l; try done. iDestruct "H'" as %[? _].
       iMod ("Hclose" with "[Harr]") as "HΦ".
-      { iSplitL. iExists arr0, ls1. iFrame "∗#%".
+      { iSplitL. iExists arr0, vs1. iFrame "∗#%".
         iPureIntro; split; try done. by right. }
-      iModIntro. wp_pures. wp_load. wp_pures.
-      rewrite Hmi. wp_pures. done.
-    - apply not_true_is_false in Hmi. rewrite Hmi.
-      destruct (decide (nx1 !!! i = m)) as [Hnx1_i | Hnx1_i]; last first.
-      + iDestruct "HAU" as "[_ Hclose]".
-        iSpecialize ("Hclose" $! false nx1).
+      iModIntro. wp_pures. done.
+    - destruct vi; try done. destruct l; try done. 
+      iDestruct "HAU" as "[Hclose _]".
+      iMod ("Hclose" with "[Harr]") as "AU".
+      { iSplitL; last by iPureIntro. iExists arr0, vs1. iFrame "∗#%". }
+      iModIntro. wp_pures. wp_bind (CmpXchg _ _ _)%E.
+      iMod "AU" as (h2 m2 nx2 k2) "[(Node&%Hi2) HAU]".
+      iDestruct "Node" as (arr2 vs2) "(#Hk2 & #Hn2 & Harr & %Len_vs2 & #Hvs2)".
+      iDestruct (mapsto_agree with "[$Hn0] [$Hn2]") as "%H'". 
+      inversion H'; subst arr2; clear H'.
+      assert (∃ vi', vs2 !! i = Some vi') as [vi' Def_vi'].
+      { apply lookup_lt_is_Some. by destruct Len_vs2 as [-> _]. } iClear "H'".
+      iDestruct ("Hvs2" with "[%]") as "H'". apply Def_vi'.
+      destruct vi'; try done.
+      + destruct vi'; try done. destruct l1; try done.
+        wp_apply (wp_cmpxchg_fail_offset _ _ _ _ _ _ (InjLV #l1) with "[Harr]"); 
+          try done.
+        { left; try done. }
+        iIntros "Harr". iDestruct "HAU" as "[Hclose _]".
         iMod ("Hclose" with "[Harr]") as "AU".
-        { iSplitL. iExists arr0, ls1. iFrame "∗#%". iPureIntro.
-          split; try done. by left. }
-        iModIntro. wp_pures. wp_load. wp_pures.
-        rewrite bool_decide_eq_false_2; last first. { by intros [=]. }
-        wp_pures. done.
-      + iDestruct "HAU" as "[Hclose _]".
-        iMod ("Hclose" with "[Harr]") as "AU".
-        { iSplitL; last by iPureIntro. iExists arr0, ls1. iFrame "∗#%". }
-        iModIntro. wp_pures. wp_load. wp_pures.
-        rewrite bool_decide_eq_true_2; last first. { by rewrite Hnx1_i. }
-        wp_pures. wp_alloc li_new as "Hnew". wp_pures.
-        wp_bind (CmpXchg _ _ _)%E.
-        iMod "AU" as (h2 m2 nx2 k2) "[(Node&%Hi2) HAU]".
-        iDestruct "Node" as (arr2 ls2) "(#Hk2 & #Hn2 & Harr & %Len_vs2 & #Hls2)".
-        iDestruct (mapsto_agree with "[$Hn0] [$Hn2]") as "%H'". 
-        inversion H'; subst arr2; clear H'.
-        assert (∃ li', ls2 !! i = Some li') as [li' Def_li'].
-        { apply lookup_lt_is_Some. by destruct Len_vs2 as [-> _]. }
-        destruct (decide (li' = li)) as [-> | Des_li].
-        * wp_apply (wp_cmpxchg_suc_offset _ _ _ _ _ _ with "[Harr]"); 
+        { iSplitL; last by iPureIntro. iExists arr0, vs2. iFrame "∗#%". }
+        iModIntro. wp_pures. by iApply "IH".
+      + destruct vi'; try done. destruct l1; try done.
+        destruct (decide (l1 = m)) as [-> | Des_l1]; last first.
+        * wp_apply (wp_cmpxchg_fail_offset _ _ _ _ _ _ (InjRV #l1) with "[Harr]"); 
             try done.
-          { by rewrite list_lookup_fmap Def_li' /=. }
-          { left; try done. }
-          iIntros "Harr". iDestruct "HAU" as "[_ Hclose]".
-          iSpecialize ("Hclose" $! true (<[i:=m']> nx2)).
-          iDestruct (mapsto_persist with "Hnew") as ">#Hnew'".
-          iDestruct ("Hls2" with "[%]") as "H''". apply Def_li'.
-          iDestruct (mapsto_agree with "H' H''") as "%H'". inversion H'.
-          iMod ("Hclose" with "[Harr]") as "HΦ".
-          { iSplitL. iExists arr0, (<[i:= li_new]> ls2). iFrame "#".
-            iSplitL. 
-            assert (((λ l : loc, #l) <$> <[i:=li_new]> ls2) = 
-                      <[i:=#li_new]> ((λ l : loc, #l) <$> ls2)) as ->.
-            { destruct Len_vs2 as [Len_vs2 _]. apply list_eq. intros i'. 
-              destruct (decide (i' = i)) as [-> | Hi'].
-              rewrite list_lookup_fmap !list_lookup_insert /=. done.
-              by rewrite fmap_length Len_vs2. by rewrite Len_vs2. 
-              rewrite list_lookup_fmap !list_lookup_insert_ne /=; try done.
-              by rewrite list_lookup_fmap. }
-            iFrame "Harr". iSplitR. { iPureIntro. by rewrite insert_length. }
-            iIntros (l j)"%Hlj". 
-            destruct (decide (j = i)) as [-> | Hj]. 
-            rewrite list_lookup_insert in Hlj. inversion Hlj. subst l.
-            rewrite -H0. 
-            assert (#((<[i:=m']> nx2 !!! i): Node) = #m') as H1'.
-            apply f_equal. by rewrite lookup_total_insert.  
-            iEval (rewrite -H1') in "Hnew'". iFrame "Hnew'". lia.
-            rewrite list_lookup_insert_ne in Hlj; try done. 
-            iClear "H' H''".
-            iDestruct ("Hls2" with "[%]") as "H'". apply Hlj. 
-            assert ((<[i:=m']> nx2 !!! j : Node) = nx2 !!! j) as H1'.
-            by rewrite lookup_total_insert_ne. iEval (rewrite -H1') in "H'". 
-            iFrame "H'". iPureIntro. repeat split; try done. by rewrite -H1. }
-          iModIntro. wp_pures. done.
-        * wp_apply (wp_cmpxchg_fail_offset _ _ _ _ _ _ #li' with "[Harr]"); 
-            try done.
-          {  by rewrite list_lookup_fmap Def_li' /=. }
           { by intros [=->]. }
           { left; try done. }
           iIntros "Harr". iDestruct "HAU" as "[Hclose _]".
           iMod ("Hclose" with "[Harr]") as "AU".
-          { iSplitL; last by iPureIntro. iExists arr0, ls2. iFrame "∗#%". }
+          { iSplitL; last by iPureIntro. iExists arr0, vs2. iFrame "∗#%". }
           iModIntro. wp_pures. by iApply "IH".
+        * wp_apply (wp_cmpxchg_suc_offset _ _ _ _ _ _ with "[Harr]"); 
+            try done.
+          { left; try done. }
+          iIntros "Harr". iDestruct "HAU" as "[_ Hclose]".
+          iSpecialize ("Hclose" $! true (<[i:=m']> nx2)).
+          iClear "Hvs0 Hvs1".
+          iMod ("Hclose" with "[Harr]") as "HΦ".
+          { iDestruct "H'" as %[? ?].
+            iSplitL. iExists arr0, (<[i:= InjRV #m']> vs2). iFrame "# Harr".
+            iSplitR. { iPureIntro. by rewrite insert_length. }
+            iIntros (v j)"%Hvj". 
+            destruct (decide (j = i)) as [-> | Hj]. 
+            rewrite list_lookup_insert in Hvj. inversion Hvj. subst v.
+            iPureIntro. split; try done.
+            assert (((<[i:=m']> nx2 !!! i): Node) = m') as H1'.
+            by rewrite lookup_total_insert. done. lia.
+            rewrite list_lookup_insert_ne in Hvj; try done.
+            iDestruct ("Hvs2" with "[%]") as "H'". apply Hvj.
+            destruct v; try done; destruct v; try done; destruct l1; try done.
+            all: try iDestruct "H'" as %[? ?]. 
+            all: try (iPureIntro; rewrite lookup_total_insert_ne; try done).
+            iPureIntro. repeat split; try done. }
+          iModIntro. wp_pures. done.
   Qed.
 
   Lemma changeNext_proph_spec Σ (Hg1 : heapGS Σ) (n m m': Node) (p: proph_id) pvs :
@@ -1021,98 +935,79 @@ Module IMPL1 : NODE_IMPL.
     iIntros "Hproph" (Φ) "AU". iLöb as "IH" forall (pvs).
     wp_lam. wp_pures. wp_bind (! _)%E.
     iMod "AU" as (h0 m0 nx0 k0) "[(Node&%Hi0) [Hclose _]]".
-    iDestruct "Node" as (arr0 ls0) "(#Hk0 & #Hn0 & Harr & %Len_vs0 & #Hls0)".
+    iDestruct "Node" as (arr0 vs0) "(#Hk0 & #Hn0 & Harr & %Len_vs0 & #Hvs0)".
     wp_load. 
     iMod ("Hclose" with "[Harr]") as "AU".
-    { iSplitL; last by iPureIntro. iExists arr0, ls0. iFrame "∗#%". }
-    iModIntro. wp_pures. wp_bind (! _)%E.
+    { iSplitL; last by iPureIntro. iExists arr0, vs0. iFrame "∗#%". }
+    iModIntro. iClear "Hvs0". wp_pures. wp_bind (! _)%E.
     iMod "AU" as (h1 m1 nx1 k1) "[(Node&%Hi1) HAU]".
-    iDestruct "Node" as (arr1 ls1) "(#Hk1 & #Hn1 & Harr & %Len_vs1 & #Hls1)".
+    iDestruct "Node" as (arr1 vs1) "(#Hk1 & #Hn1 & Harr & %Len_vs1 & #Hvs1)".
     iDestruct (mapsto_agree with "[$Hn0] [$Hn1]") as "%H'". 
     inversion H'; subst arr1; clear H'.
-    assert (∃ li, ls1 !! 0 = Some li) as [li Def_li].
+    assert (∃ vi, vs1 !! 0 = Some vi) as [vi Def_vi].
     { apply lookup_lt_is_Some. by destruct Len_vs1 as [-> _]. }  
     wp_apply (wp_load_offset _ _ _ (DfracOwn (pos_to_Qp 1)) _ 
-        _ #li with "[Harr]"); try done.
-    { by rewrite list_lookup_fmap Def_li /=. }
+        _ vi with "[Harr]"); try done.
     iIntros "Harr".
-    iDestruct ("Hls1" with "[%]") as "H'". apply Def_li.
-    destruct (decide (m1 !!! 0 = true)) as [Hmi | Hmi].
+    iDestruct ("Hvs1" with "[%]") as "H'". apply Def_vi.
+    destruct vi; try done.
     - iDestruct "HAU" as "[_ Hclose]".
       iSpecialize ("Hclose" $! false nx1).
+      destruct vi; try done. destruct l; try done. iDestruct "H'" as %[? _].
       iMod ("Hclose" with "[Harr Hproph]") as "HΦ".
-      { iFrame. iSplitL. iExists arr0, ls1. iFrame "∗#%".
+      { iFrame. iSplitL. iExists arr0, vs1. iFrame "∗#%".
         iPureIntro; split; try done. repeat split; try done. by right. }
-      iModIntro. wp_pures. wp_load. wp_pures.
-      rewrite Hmi. wp_pures. done.
-    - apply not_true_is_false in Hmi. rewrite Hmi.
-      destruct (decide (nx1 !!! 0 = m)) as [Hnx1_i | Hnx1_i]; last first.
-      + iDestruct "HAU" as "[_ Hclose]".
-        iSpecialize ("Hclose" $! false nx1).
-        iMod ("Hclose" with "[Harr Hproph]") as "AU".
-        { iFrame. iSplitL. iExists arr0, ls1. iFrame "∗#%". iPureIntro.
-          repeat split; try done. by left. }
-        iModIntro. wp_pures. wp_load. wp_pures.
-        rewrite bool_decide_eq_false_2; last first. { by intros [=]. }
-        wp_pures. done.
-      + iDestruct "HAU" as "[Hclose _]".
-        iMod ("Hclose" with "[Harr]") as "AU".
-        { iSplitL; last by iPureIntro. iExists arr0, ls1. iFrame "∗#%". }
-        iModIntro. wp_pures. wp_load. wp_pures.
-        rewrite bool_decide_eq_true_2; last first. { by rewrite Hnx1_i. }
-        wp_pures. wp_alloc li_new as "Hnew". wp_pures.
-        wp_bind (Resolve _ _ _)%E. 
-        iMod "AU" as (h2 m2 nx2 k2) "[(Node&%Hi2) HAU]".
-        iDestruct "Node" as (arr2 ls2) "(#Hk2 & #Hn2 & Harr & %Len_vs2 & #Hls2)".
-        iDestruct (mapsto_agree with "[$Hn0] [$Hn2]") as "%H'". 
-        inversion H'; subst arr2; clear H'.
-        destruct ls2 as [|li' ls2'] eqn: Def_ls2. 
-        { rewrite /= in Len_vs2. exfalso; lia. }
-        assert (ls2 !! 0 = Some li') as Def_li'.
-        { by rewrite Def_ls2 /=. }
-        assert (((λ l : loc, #l) <$> li' :: ls2') = 
-          #li' :: ((λ l : loc, #l) <$> ls2')) as ->.
-        { by rewrite fmap_cons. } rewrite array_cons. 
-        iDestruct "Harr" as "(Harr0 & Harr)".
-        assert (arr0 +ₗ 0%nat = arr0) as ->. { by rewrite Loc.add_0. }
-        destruct (decide (li' = li)) as [-> | Des_li].
-        * wp_apply (wp_resolve_cmpxchg_suc with "[$Harr0 $Hproph]").
-          { by left. }
-          iIntros "H''". iDestruct "H''" as (pvs')"(%Hpvs' & Hproph & Harr0)".
-          iDestruct "HAU" as "[_ Hclose]".
-          iSpecialize ("Hclose" $! true (<[0:=m']> nx2)).
-          iDestruct (mapsto_persist with "Hnew") as ">#Hnew'".
-          iDestruct ("Hls2" with "[%]") as "H''". rewrite -Def_ls2. apply Def_li'.
-          iDestruct (mapsto_agree with "H' H''") as "%H'". inversion H'.
-          iMod ("Hclose" with "[Harr Harr0 Hproph]") as "HΦ".
-          { iFrame "Hproph". iSplitL. iExists arr0, (<[0:= li_new]> ls2). iFrame "#".
-            iSplitL. assert (((λ l : loc, #l) <$> <[0:=li_new]> ls2) = 
-              #li_new :: ((λ l : loc, #l) <$> ls2')) as ->.
-            { rewrite Def_ls2 /=. apply f_equal. done. } 
-            rewrite array_cons. iFrame. 
-            iSplitR. { iPureIntro. by rewrite insert_length Def_ls2. }
-            iIntros (l j)"%Hlj". destruct (decide (j = 0)) as [-> | Hj].
-            rewrite list_lookup_insert in Hlj. inversion Hlj. subst l.
-            assert (m2 !!! 0%nat = false) as -> by done.
-            assert ((<[0%nat:=m']> nx2 !!! 0%nat : loc) = m') as ->.
-            by rewrite lookup_total_insert.
-            rewrite H1; try done. destruct Len_vs2 as [Len_vs2 _]. 
-            by rewrite Def_ls2 Len_vs2.
-            assert ((<[0%nat:=m']> nx2 !!! j : loc) = nx2 !!! j) as ->.
-            by rewrite lookup_total_insert_ne.
-            rewrite list_lookup_insert_ne in Hlj; try done.
-            iClear "H' H''".
-            iDestruct ("Hls2" with "[%]") as "H'". rewrite -Def_ls2. apply Hlj.
-            iFrame "#". iPureIntro. repeat split; try done. by rewrite -H1.
-            exists #li. rewrite Hpvs'. clear; set_solver. }
-          iModIntro. wp_pures. done.
+      iModIntro. wp_pures. done.
+    - destruct vi; try done. destruct l; try done. 
+      iDestruct "HAU" as "[Hclose _]".
+      iMod ("Hclose" with "[Harr]") as "AU".
+      { iSplitL; last by iPureIntro. iExists arr0, vs1. iFrame "∗#%". }
+      iModIntro. iClear "Hvs1". wp_pures. wp_bind (Resolve _ _ _)%E.
+      iMod "AU" as (h2 m2 nx2 k2) "[(Node&%Hi2) HAU]".
+      iDestruct "Node" as (arr2 vs2) "(#Hk2 & #Hn2 & Harr & %Len_vs2 & #Hvs2)".
+      iDestruct (mapsto_agree with "[$Hn0] [$Hn2]") as "%H'". 
+      inversion H'; subst arr2; clear H'.
+      destruct vs2 as [|vi' vs2'] eqn: Def_vs2.
+      { clear -Len_vs2. exfalso. rewrite /= in Len_vs2. lia. } rewrite -Def_vs2.
+      assert (vs2 !! 0 = Some vi') as Def_vi'. { rewrite Def_vs2 /=. done. }
+      iClear "H'". iDestruct ("Hvs2" with "[%]") as "H'". apply Def_vi'.
+      iEval (rewrite Def_vs2 array_cons) in "Harr".
+      iDestruct "Harr" as "(Harr0 & Harr)".
+      assert (arr0 +ₗ 0%nat = arr0) as ->. { by rewrite Loc.add_0. }
+      destruct vi'; try done.
+      + destruct vi'; try done. destruct l1; try done.
+        wp_apply (wp_resolve_cmpxchg_fail with "[$Harr0 $Hproph]").
+        { intros H'. inversion H'. }
+        { left; try done. }
+        iIntros "H''". iDestruct "H''" as (pvs')"(%Hpvs' & Hproph & Harr0)".
+        iDestruct "HAU" as "[Hclose _]". iMod ("Hclose" with "[Harr Harr0]") as "AU".
+        { iSplitL; last by iPureIntro. iExists arr0, (InjLV #l1 :: vs2'). 
+          iFrame "∗#%". rewrite Def_vs2. done. }
+        iModIntro. wp_pures. iApply ("IH" with "[$Hproph] [AU]"); try done.
+        iAuIntro. rewrite /atomic_acc /=. iClear "#". 
+        iMod "AU" as (h3 m3 nx3 k3)"[H' H'']". iModIntro.
+        iExists h3, m3, nx3, k3. iFrame "H'". iSplit.
+        ** iDestruct "H''" as "[H'' _]". iApply "H''".
+        ** iDestruct "H''" as "[_ H'']". iIntros (res nx3' prf pvs'').
+          iIntros "(Node & Hproph & %Hprf & Hres)". 
+          iSpecialize ("H''" $! res nx3' (((InjLV #l1, #false)%V, #()) :: prf) pvs'').
+          iMod ("H''" with "[Node Hproph Hres]") as "HΦ"; try done.
+          iFrame "Node Hproph". iSplitR. iPureIntro. 
+          rewrite Forall_cons; split; try done. by exists (InjLV #l1).
+          destruct res; iDestruct "Hres" as "%H'"; iPureIntro; 
+            repeat split; try apply H'. destruct H' as (_&_&_&[v1 Def_pvs']).
+          rewrite Def_pvs' in Hpvs'. exists v1. rewrite Hpvs'. done.
+          destruct H' as (_&_&Def_pvs'). rewrite Def_pvs' in Hpvs'.
+          rewrite Hpvs'. clear; set_solver.
+      + destruct vi'; try done. destruct l1; try done.
+        destruct (decide (l1 = m)) as [-> | Des_l1]; last first.
         * wp_apply (wp_resolve_cmpxchg_fail with "[$Harr0 $Hproph]").
-          { by intros [=->]. }
-          { by left. }
+          { intros H'. inversion H'. done. }
+          { left; try done. }
           iIntros "H''". iDestruct "H''" as (pvs')"(%Hpvs' & Hproph & Harr0)".
-          iDestruct "HAU" as "[Hclose _]".
-          iMod ("Hclose" with "[Harr Harr0]") as "AU".
-          { iSplitL; last by iPureIntro. iExists arr0, (li' :: ls2'). iFrame "∗#%". }
+          iDestruct "HAU" as "[Hclose _]". iMod ("Hclose" with "[Harr Harr0]") as "AU".
+          { iSplitL; last by iPureIntro. iExists arr0, (InjRV #l1 :: vs2'). 
+            iFrame "∗#%". rewrite Def_vs2. done. }
           iModIntro. wp_pures. iApply ("IH" with "[$Hproph] [AU]"); try done.
           iAuIntro. rewrite /atomic_acc /=. iClear "#". 
           iMod "AU" as (h3 m3 nx3 k3)"[H' H'']". iModIntro.
@@ -1120,15 +1015,41 @@ Module IMPL1 : NODE_IMPL.
           ** iDestruct "H''" as "[H'' _]". iApply "H''".
           ** iDestruct "H''" as "[_ H'']". iIntros (res nx3' prf pvs'').
             iIntros "(Node & Hproph & %Hprf & Hres)". 
-            iSpecialize ("H''" $! res nx3' (((#li', #false)%V, #()) :: prf) pvs'').
+            iSpecialize ("H''" $! res nx3' (((InjRV #l1, #false)%V, #()) :: prf) pvs'').
             iMod ("H''" with "[Node Hproph Hres]") as "HΦ"; try done.
             iFrame "Node Hproph". iSplitR. iPureIntro. 
-            rewrite Forall_cons; split; try done. by exists #li'.
+            rewrite Forall_cons; split; try done. by exists (InjRV #l1).
             destruct res; iDestruct "Hres" as "%H'"; iPureIntro; 
               repeat split; try apply H'. destruct H' as (_&_&_&[v1 Def_pvs']).
             rewrite Def_pvs' in Hpvs'. exists v1. rewrite Hpvs'. done.
             destruct H' as (_&_&Def_pvs'). rewrite Def_pvs' in Hpvs'.
             rewrite Hpvs'. clear; set_solver.
+        * wp_apply (wp_resolve_cmpxchg_suc with "[$Harr0 $Hproph]").
+          { by left. }
+          iIntros "H''". iDestruct "H''" as (pvs')"(%Hpvs' & Hproph & Harr0)".
+          iDestruct "HAU" as "[_ Hclose]".
+          iSpecialize ("Hclose" $! true (<[0:=m']> nx2)).
+          iMod ("Hclose" with "[Harr Harr0 Hproph]") as "HΦ".
+          { iDestruct "H'" as %[? ?]. iFrame "Hproph".
+            iSplitL. iExists arr0, (<[0:= InjRV #m']> vs2). iFrame "#".
+            iSplitL. assert (<[0:=InjRV #m']> vs2 = InjRV #m' :: vs2') as ->.
+            { rewrite Def_vs2 /=. apply f_equal. done. }
+            rewrite array_cons. iFrame. 
+            iSplitR. { iPureIntro. by rewrite insert_length Def_vs2. }
+            iIntros (v j)"%Hvj". destruct (decide (j = 0)) as [-> | Hj]. 
+            rewrite list_lookup_insert in Hvj. inversion Hvj. subst v.
+            assert (m2 !!! 0%nat = false) as -> by done.
+            assert ((<[0%nat:=m']> nx2 !!! 0%nat : loc) = m') as ->.
+            by rewrite lookup_total_insert. by iPureIntro. 
+            destruct Len_vs2 as [Len_vs2 _]. by rewrite Def_vs2 Len_vs2.
+            assert ((<[0%nat:=m']> nx2 !!! j : loc) = nx2 !!! j) as ->.
+            by rewrite lookup_total_insert_ne. 
+            rewrite list_lookup_insert_ne in Hvj; try done.
+            iDestruct ("Hvs2" with "[%]") as "H'". apply Hvj.
+            iFrame "#". iPureIntro. repeat split; try done.
+            exists (InjRV #m). rewrite Hpvs'. clear; set_solver. }
+          iModIntro. wp_pures. done.
   Qed.
 
-End IMPL1.
+
+End IMPL2.
