templates/lockfree/herlihy.v
@@ -130,7 +130,7 @@ Module HERLIHY_SPEC <: TRAVERSE_SPEC.
     iIntros (Φ) "!# (#Htr&#Marked_p&#Htr0) Hpost". wp_lam. wp_pure credit: "Hc". 
     wp_pures. awp_apply findNext_spec.
     iInv "HInv" as (M0 T0 s0) "(>Ds & >%Habs0 & >Hist & Help & >Templ)".
-    iDestruct "Templ" as (hd' tl')"(HR & SShot0 & Res & %PT0 & %Trans_M0)".
+    iDestruct "Templ" as (hd' tl' γ_ks)"(HR & SShot0 & Res & %PT0 & %Trans_M0)".
     iAssert (⌜hd' = hd ∧ tl' = tl⌝)%I with "[HR]" as %[-> ->]. 
     { iDestruct (mapsto_agree with "[$HR] [$HR']") as %[=]. by iPureIntro. }
     iDestruct "Res" as "(GKS & Nodes & Nodes_KS)".
@@ -152,7 +152,7 @@ Module HERLIHY_SPEC <: TRAVERSE_SPEC.
     { iFrame "Node_c %". }
     iAaccIntro with "Hpre".
     { iIntros "(Node_c & _)". iModIntro. iFrame "Hpost Hc".
-      iNext; iExists M0, T0, s0. iFrame "∗%#". iExists hd, tl. iFrame "∗%#". 
+      iNext; iExists M0, T0, s0. iFrame "∗%#". iExists hd, tl, γ_ks. iFrame "∗%#". 
       rewrite (big_sepS_delete _ (FP s0) c); last by eauto. 
       iFrame "Nodes_rest". iFrame. }
     iIntros (m cn) "(Node_c & %Mark_c0 & %Next_c0)".
@@ -221,13 +221,13 @@ Module HERLIHY_SPEC <: TRAVERSE_SPEC.
       rewrite bool_decide_eq_true in Hbool. clear -Hbool; set_solver.
       rewrite bool_decide_eq_false in Hbool. clear -Hbool; set_solver. }
     iModIntro. iSplitR "Hpost Hc".
-    { iNext. iExists M0, T0, s0. iFrame "∗%". iExists hd, tl. iFrame "∗%".
+    { iNext. iExists M0, T0, s0. iFrame "∗%". iExists hd, tl, γ_ks. iFrame "∗%".
       rewrite (big_sepS_delete _ (FP s0) c); last by eauto.
       iFrame "Nodes_rest". iFrame. }
     destruct m; wp_pures. 
-    - awp_apply changeNext_spec; try done.
+    - awp_apply changeNext_spec; try done. clear γ_ks.
       iInv "HInv" as (M1 T1 s1) "(>Ds & >%Habs1 & >Hist & Help & >Templ)".
-      iDestruct "Templ" as (hd' tl')"(HR & SShot1 & Res & %PT1 & %Trans_M1)".
+      iDestruct "Templ" as (hd' tl' γ_ks)"(HR & SShot1 & Res & %PT1 & %Trans_M1)".
       iAssert (⌜hd' = hd ∧ tl' = tl⌝)%I with "[HR]" as %[-> ->]. 
       { iDestruct (mapsto_agree with "[$HR] [$HR']") as %[=]. by iPureIntro. }
       iDestruct "Res" as "(GKS & Nodes & Nodes_KS)".
@@ -249,7 +249,7 @@ Module HERLIHY_SPEC <: TRAVERSE_SPEC.
       { iFrame "Node_p %". }
       iAaccIntro with "Hpre".
       { iIntros "(Node_p&_)". iModIntro. iFrame "Hpost Hc".
-        iNext; iExists M1, T1, s1. iFrame "∗%#". iExists hd, tl. iFrame "∗%#". 
+        iNext; iExists M1, T1, s1. iFrame "∗%#". iExists hd, tl, γ_ks. iFrame "∗%#". 
         rewrite (big_sepS_delete _ (FP s1) p); last by eauto. iFrame. }
       iIntros (success next') "(Node_p & Hsuccess)".
       iApply (lc_fupd_add_later with "Hc"). iNext. 
@@ -735,7 +735,7 @@ Module HERLIHY_SPEC <: TRAVERSE_SPEC.
           iModIntro. iSplitR "Hpost".
           { iNext. iExists M1', (T1+1), s1'. iFrame "∗#%". 
             iSplitR. iPureIntro. rewrite /M1'. by rewrite lookup_total_insert.
-            iExists hd, tl. iFrame "∗#%".
+            iExists hd, tl, γ_ks. iFrame "∗#%".
             iPureIntro; rewrite /M1'; split.
             - intros t Ht. destruct (decide (t = T1+1)) as [-> | Ht'].
               + by rewrite lookup_total_insert.
@@ -754,7 +754,7 @@ Module HERLIHY_SPEC <: TRAVERSE_SPEC.
             by rewrite lookup_insert Next_p1. by rewrite lookup_insert_ne. }
           rewrite Hnext'.
           iModIntro. iSplitR "Hpost".
-          { iNext. iExists M1, T1, s1. iFrame "∗#%". iExists hd, tl. iFrame "∗#%".
+          { iNext. iExists M1, T1, s1. iFrame "∗#%". iExists hd, tl, γ_ks. iFrame "∗#%".
             rewrite (big_sepS_delete _ (FP s1) p); try done. iFrame. }
           wp_pures.
           iApply "IH"; try done. iFrame "Htr Marked_p". iIntros "%"; try done.
@@ -905,7 +905,7 @@ Module HERLIHY_SPEC <: TRAVERSE_SPEC.
           iModIntro. iSplitR "Hpost".
           { iNext. iExists M1', (T1+1), s1'. iFrame "∗#%".
             iSplitR. iPureIntro. rewrite /M1'. by rewrite lookup_total_insert.
-            iExists hd, tl. iFrame "∗#%".
+            iExists hd, tl, γ_ks. iFrame "∗#%".
             iPureIntro; rewrite /M1'; split.
             - intros t Ht. destruct (decide (t = T1+1)) as [-> | Ht'].
               + by rewrite lookup_total_insert.
@@ -920,13 +920,13 @@ Module HERLIHY_SPEC <: TRAVERSE_SPEC.
           iApply "IH"; try done. iFrame "Htr' Marked_p". iIntros "%"; try done.
       + iDestruct "Hsuccess" as %[Hcond ->].
         iModIntro. iSplitR "Hpost".
-        { iNext. iExists M1, T1, s1. iFrame "∗%". iExists hd, tl. iFrame "∗%".
+        { iNext. iExists M1, T1, s1. iFrame "∗%". iExists hd, tl, γ_ks. iFrame "∗%".
           rewrite (big_sepS_delete _ (FP s1) p); last by eauto.
           iFrame "Nodes_rest". iFrame. }
         wp_pures. iSpecialize ("Hpost" $! None). by iApply "Hpost".
-    - awp_apply getKey_spec. 
+    - awp_apply getKey_spec. clear γ_ks.
       iInv "HInv" as (M1 T1 s1) "(>Ds & >%Habs1 & >Hist & Help & >Templ)".
-      iDestruct "Templ" as (hd' tl')"(HR & SShot1 & Res & %PT1 & %Trans_M1)".
+      iDestruct "Templ" as (hd' tl' γ_ks)"(HR & SShot1 & Res & %PT1 & %Trans_M1)".
       iAssert (⌜hd' = hd ∧ tl' = tl⌝)%I with "[HR]" as %[-> ->]. 
       { iDestruct (mapsto_agree with "[$HR] [$HR']") as %[=]. by iPureIntro. }
       iDestruct "Res" as "(GKS & Nodes & Nodes_KS)".
@@ -937,7 +937,7 @@ Module HERLIHY_SPEC <: TRAVERSE_SPEC.
       iDestruct "Nodes" as "(Node_c & Nodes_rest)".
       iAaccIntro with "Node_c".
       { iIntros "Node_c". iModIntro. iFrame "Hpost Hc".
-        iNext; iExists M1, T1, s1. iFrame "∗%#". iExists hd, tl. iFrame "∗%#".
+        iNext; iExists M1, T1, s1. iFrame "∗%#". iExists hd, tl, γ_ks. iFrame "∗%#".
         rewrite (big_sepS_delete _ (FP s1) c); last by eauto. iFrame. }
       iIntros "Node_c". set kc := Key s1 c.
       iPoseProof (snapshot_current with "[%] [#] [$Hist]") 
@@ -946,7 +946,7 @@ Module HERLIHY_SPEC <: TRAVERSE_SPEC.
       { apply leibniz_equiv in Habs1. rewrite -Habs1.
         iPoseProof (key_eq_2 with "[%] [$Hist] [$Past_s0] [%]") as "->"; try done. }
       iModIntro. iSplitR "Hpost".
-      { iNext. iExists M1, T1, s1. iFrame "∗%". iExists hd, tl. iFrame "∗%".
+      { iNext. iExists M1, T1, s1. iFrame "∗%". iExists hd, tl, γ_ks. iFrame "∗%".
         rewrite (big_sepS_delete _ (FP s1) c); last by eauto.
         iFrame "Nodes_rest". iFrame. }
       wp_pures.
@@ -1023,7 +1023,7 @@ Module HERLIHY_SPEC <: TRAVERSE_SPEC.
     wp_pures. wp_bind (findNext _ _)%E. 
     awp_apply findNext_spec.
     iInv "HInv" as (M0 T0 s0) "(>Ds & >%Habs0 & >Hist & Help & >Templ)".
-    iDestruct "Templ" as (hd' tl') "(HR & SShot0 & Res & %PT0 & %Trans_M0)".
+    iDestruct "Templ" as (hd' tl' γ_ks) "(HR & SShot0 & Res & %PT0 & %Trans_M0)".
     iAssert (⌜hd' = hd ∧ tl' = tl⌝)%I with "[HR]" as %[-> ->]. 
     { iDestruct (mapsto_agree with "[$HR] [$HR']") as %[=]. by iPureIntro. }
     iDestruct "Res" as "(GKS & Nodes & Nodes_KS)".
@@ -1051,7 +1051,7 @@ Module HERLIHY_SPEC <: TRAVERSE_SPEC.
     { iFrame "Node_p %". }
     iAaccIntro with "Hpre".    
     { iIntros "(Node_p&_)". iModIntro. iFrame "Hpost Hpreds Hsuccs".
-      iNext; iExists M0, T0, s0. iFrame "∗%#". iExists hd, tl. iFrame "∗%#". 
+      iNext; iExists M0, T0, s0. iFrame "∗%#". iExists hd, tl, γ_ks. iFrame "∗%#". 
       rewrite (big_sepS_delete _ (FP s0) p); last by eauto. iFrame. }
     iIntros (m c) "(Node_p & %Mark_p0 & %Next_p0)".
     iAssert (⌜per_tick_inv hd tl s0⌝)%I as %PT_s0.
@@ -1152,7 +1152,7 @@ Module HERLIHY_SPEC <: TRAVERSE_SPEC.
       - iModIntro. iFrame. iIntros "%"; try done. }
     
     iModIntro. iSplitR "Hpreds Hsuccs Hpost Hj".
-    { iNext. iExists M0, T0, s0. iFrame "∗%". iExists hd, tl. iFrame "∗%".
+    { iNext. iExists M0, T0, s0. iFrame "∗%". iExists hd, tl, γ_ks. iFrame "∗%".
       rewrite (big_sepS_delete _ (FP s0) p); last by eauto. iFrame. }
     wp_pures. wp_apply traverse_i_spec; try done. iFrame "Htr Htr0 Marked_p".
     iIntros (ores) "Hores".
@@ -1217,7 +1217,7 @@ Module HERLIHY_SPEC <: TRAVERSE_SPEC.
       & %Hps0_L & %Hss0_L & #Hj)".
     wp_lam. wp_pures. iApply fupd_wp.
     iInv "HInv" as (M0 T0 s0) "(>Ds & >%Habs0 & >Hist & Help & >Templ)".
-    iDestruct "Templ" as (hd' tl')"(HR & SShot0 & Res & %PT0 & %Trans_M0)".
+    iDestruct "Templ" as (hd' tl' γ_ks)"(HR & SShot0 & Res & %PT0 & %Trans_M0)".
     iAssert (⌜hd' = hd ∧ tl' = tl⌝)%I with "[HR]" as %[-> ->]. 
     { iDestruct (mapsto_agree with "[$HR] [$HR']") as %[=]. by iPureIntro. }
     iAssert (⌜per_tick_inv hd tl s0⌝)%I as %PT_s0.
@@ -1231,7 +1231,7 @@ Module HERLIHY_SPEC <: TRAVERSE_SPEC.
     { iExists s0. iFrame "Past_s0". iPureIntro. destruct PT_s0 as (PT&_).
       destruct PT as (H'&_&_&H''&_). split. set_solver. apply H''. lia. }
     iModIntro. iSplitR "Hpreds Hsuccs Hpost".
-    { iNext. iExists M0, T0, s0. iFrame "∗%". iExists hd, tl. iFrame "∗%". }
+    { iNext. iExists M0, T0, s0. iFrame "∗%". iExists hd, tl, γ_ks. iFrame "∗%". }
     iModIntro.      
     wp_apply (traverse_pop_spec with "[] [] [] [] [] [Hpreds Hsuccs]"); try done.
     iFrame "Hpreds Hsuccs Hj %". iIntros (ores ps ss b)"Hores".
@@ -1289,7 +1289,7 @@ Module HERLIHY_SPEC <: TRAVERSE_SPEC.
     iApply array_repeat. iPureIntro; lia.
     iNext. iIntros (succs) "Hsuccs". wp_pures. iApply fupd_wp.
     iInv "HInv" as (M0 T0 s0) "(>Ds & >%Habs0 & >Hist & Help & >Templ)".
-    iDestruct "Templ" as (hd' tl')"(HR & SShot0 & Res & %PT0 & %Trans_M0)".
+    iDestruct "Templ" as (hd' tl' γ_ks)"(HR & SShot0 & Res & %PT0 & %Trans_M0)".
     iAssert (⌜hd' = hd ∧ tl' = tl⌝)%I with "[HR]" as %[-> ->]. 
     { iDestruct (mapsto_agree with "[$HR] [$HR']") as %[=]. by iPureIntro. }
     iAssert (⌜per_tick_inv hd tl s0⌝)%I as %PT_s0.
@@ -1303,7 +1303,7 @@ Module HERLIHY_SPEC <: TRAVERSE_SPEC.
     { iExists s0. iFrame "Past_s0". iPureIntro. destruct PT_s0 as (PT&_).
       destruct PT as (H'&_&_&H''&_). split. set_solver. apply H''. lia. }
     iModIntro. iSplitR "Hpreds Hsuccs Hpost".
-    { iNext. iExists M0, T0, s0. iFrame "∗%". iExists hd, tl. iFrame "∗%". }
+    { iNext. iExists M0, T0, s0. iFrame "∗%". iExists hd, tl, γ_ks. iFrame "∗%". }
     iModIntro.      
     wp_apply (traverse_rec_spec with "[] [] [] [] [] [Hpreds Hsuccs]"); try done.
     iFrame "Hpreds Hsuccs".
