templates/lockfree/skiplist_spec.v
@@ -11,6 +11,7 @@ From iris.heap_lang.lib Require Import nondet_bool.
 From iris.bi.lib Require Import fractional.
 Set Default Proof Using "All".
 From iris.bi.lib Require Import fractional.
+Require Import multiset_flows keyset_ra2.
 Require Export skiplist_search skiplist_insert skiplist_delete hindsight_proof.
 
 Module SKIPLIST_SPEC : HINDSIGHT_SPEC.
@@ -21,24 +22,307 @@ Module SKIPLIST_SPEC : HINDSIGHT_SPEC.
   Module DEFS := TR_SPEC.SK_UTIL.DEFS.
   Export TR_SPEC TR_SPEC.SK_UTIL TR_SPEC.SK_UTIL.SK TR_SPEC.SK_UTIL.DEFS.
   Export TR_SPEC.SK_UTIL.SK.TR.NODE TR_SPEC.SK_UTIL.SK.TR.
+
+  Lemma init_spec Σ Hg1 Hg2 :
+    {{{ True }}} init #() 
+    {{{ (r: Node) (s : snapshot), RET #r; ds_inv Σ Hg1 Hg2 r {[0 := s]} 0 s }}}.
+  Proof.
+    iIntros (Φ) "_ Hpost". wp_lam. wp_apply createTail_spec; try done.
+    iIntros (tl mt) "(Node_tl & %Dom_mt & %Mt_i)". 
+    wp_pures. wp_apply createHead_spec; try done.
+    iIntros (hd mh nh) "(Node_hd & %Dom_mh & %Dom_nh & %Mh_i & %Nh_i)".
+    wp_pures. wp_alloc r as "HR". wp_pures. 
+    iDestruct (mapsto_persist with "HR") as ">#HR".
+    set N : gset Node := {[ hd; tl ]}.
+    set C : gset nat := {[ 0; W ]}.
+    set H : gmap Node nat := {[ hd := L; tl := L ]}.
+    set Mk : gmap Node MarkT := {[ hd := mh; tl := mt ]}.
+    set Nx : gmap Node NextT := {[ hd := nh; tl := ∅ ]}.
+    set Ky : gmap Node nat := {[ hd := 0; tl := W ]}.
+    
+    assert (∃ ks : nzmap nat nat, (dom ks = gset_seq 1 W) ∧ (∀ k, ks !!! k ≤ 1))
+      as [ks [Dom_ks Def_ks]]. 
+    { set S : gset nat := gset_seq 1 W.
+      set ks := let f := λ k res, <<[k := 1]>> res in set_fold f ∅ S.
+      assert (∀ k, (k ∈ S → ks !!! k = 1) ∧ (k ∉ S → ks !!! k = 0)) as H'.
+      { set P := λ (m' : nzmap nat nat) (X : gset nat), 
+          ∀ k, (k ∈ X → m' !!! k = 1) ∧ (k ∉ X → m' !!! k = 0).
+        apply (set_fold_ind_L P); try done.
+        intros k X res Hkx HP. rewrite /P. rewrite /P in HP.
+        intros k'. rewrite elem_of_union elem_of_singleton. split.
+        intros [-> | Hk']. rewrite nzmap_lookup_total_insert. done.
+        rewrite nzmap_lookup_total_insert_ne. apply HP. done. 
+        clear -Hkx Hk'; set_solver. intros H'. 
+        rewrite nzmap_lookup_total_insert_ne. apply HP. intros ?. apply H'.
+        by right. intros ->. apply H'. by left. }
+      exists ks. split. apply set_eq_subseteq. split. intros k Hk.
+      rewrite nzmap_elem_of_dom_total in Hk. destruct (decide (k ∈ S)); try done.
+      apply H' in n. rewrite n in Hk. rewrite /ccmunit /= /nat_unit in Hk. lia.
+      intros k Hk. apply H' in Hk. rewrite nzmap_elem_of_dom_total Hk.
+      rewrite /ccmunit /= /nat_unit. lia. intros k. 
+      destruct (decide (k ∈ S)) as [H'' | H'']; apply H' in H''; lia. }
+    set ks' := <<[ 0 := 1 ]>> ks.
+    set Ih : multiset_flowint_ur nat := 
+      int {| infR := {[hd := ks']}; outR := <<[ tl := ks ]>> ∅ |}.
+    set It : multiset_flowint_ur nat := 
+      int {| infR := {[tl := ks]}; outR := ∅ |}.
+    set I : gmap Node (multiset_flowint_ur nat) := {[ hd := Ih; tl := It ]}.
+    set s : snapshot := (N, C, H, Mk, Nx, Ky, I).
+
+    assert (snapshot_constraints s) as SShot.
+    { exists N, C, H, Mk, Nx, Ky, I. rewrite /s. split; try done.
+      rewrite /H /Mk /Nx /Ky /I /N /= /= !dom_insert_L !dom_empty_L.
+      repeat split. all: set_solver. }
+
+    assert (W > 0) as HW. { apply W_gt_0. } 
+    assert (L > 1) as HL. { apply L_gt_1. }
+    iAssert (⌜hd ≠ tl⌝)%I as %hd_neq_tl.
+    { destruct (decide (hd = tl)) as [-> | ?]; try done. iExFalso.
+      iApply (node_sep_star with "Node_tl Node_hd"). }
+    
+    iMod (own_alloc (● prodKS (KS, C) ⋅ ◯ prodKS (KS, C))) as (γ_ks)"HKS".
+    { rewrite auth_both_valid_discrete. split; try done. 
+      rewrite /valid /cmra_valid /= /ucmra_valid /= /C /KS.
+      intros x. rewrite elem_of_union !elem_of_singleton elem_of_gset_seq. lia. }
+
+    iDestruct "HKS" as "(HKS & Hks)". 
+    assert (prodKS (KS, C) = prodKS ({[0]}, {[0]}) ⋅ prodKS (KS ∖ {[0]}, {[W]}))
+      as H'.
+    { assert (KS = {[0]} ∪ (KS ∖ {[0]})) as H'.
+      { apply set_eq_subseteq. split. intros x. destruct (decide (x = 0)) as [-> | Hx0].
+        clear; set_solver. intros Hx. rewrite elem_of_union. right. set_solver.
+        intros x. rewrite elem_of_union elem_of_singleton.
+        intros [-> | Hx]. rewrite /KS elem_of_gset_seq. lia. clear -Hx; set_solver. }
+      assert (C = {[0]} ∪ {[W]}) as -> by set_solver. rewrite {1}H'. symmetry.
+      apply (ksRAT_prodKS_op {[0]} (KS ∖ {[0]}) {[0]} {[W]}).
+      apply ksRAT_valid_composable. repeat split. rewrite /valid /=. done.
+      rewrite /valid /=. rewrite /KS. intros x. rewrite elem_of_difference.
+       rewrite elem_of_gset_seq !elem_of_singleton. lia. rewrite /=. clear; set_solver. }
+    iEval (rewrite H') in "Hks". clear H'. iDestruct "Hks" as "(Hksh & Hkst)".
+    assert (∀ i, i < L → Mark s hd !! i = Some false) as Mark_hd.
+    { rewrite /Mark /s /Mk lookup_insert. done. }
+    assert (∀ i, i < L → Mark s tl !! i = Some false) as Mark_tl.
+    { rewrite /Mark /s /Mk lookup_insert_ne; try done. by rewrite lookup_insert. }
+    assert (Key s hd = 0) as Key_hd. { by rewrite /s /Key /Ky /= lookup_insert. }
+    assert (Key s tl = W) as Key_tl. 
+    { rewrite /s /Key /Ky /= lookup_insert_ne; try done. by rewrite lookup_insert. }
+    assert (Content s hd = {[0]}) as Content_hd.
+    { rewrite /Content Key_hd /Marki lookup_total_alt Mark_hd /=. done. lia. }
+    assert (Content s tl = {[W]}) as Content_tl.
+    { rewrite /Content Key_tl /Marki lookup_total_alt Mark_tl /=. done. lia. }
+    assert (FI s hd = Ih) as FI_hd.
+    { rewrite /FI /s /I lookup_insert. done.  }
+    assert (FI s tl = It) as FI_tl.
+    { rewrite /FI /s /I lookup_insert_ne; try done. rewrite lookup_insert. done. }
+    assert (dom Ih = {[hd]}) as Dom_Ih.
+    { rewrite /dom /flowint_dom /Ih /= dom_insert_L. set_solver. }
+    assert (dom It = {[tl]}) as Dom_It.
+    { rewrite /dom /flowint_dom /It /= dom_insert_L. set_solver. }
+    assert (ks ≠ 0%CCM) as ks_neq_0.
+    { rewrite /ccmunit /ccm_unit /= /lift_unit.
+      intros H'. rewrite nzmap_eq in H'. pose proof H' W as H'.
+      rewrite nzmap_lookup_empty -nzmap_elem_of_dom_total2 in H'.
+      apply H'. rewrite Dom_ks elem_of_gset_seq. lia. }
+    assert (dom (out_map Ih) = {[tl]}) as Domout_Ih.
+    { rewrite /Ih /=. apply leibniz_equiv. rewrite nzmap_dom_insert_nonzero; try done.
+      rewrite /dom. set_solver. }
+    assert (dom (out_map It) = ∅) as Domout_It.
+    { rewrite /It /=. set_solver. }
+    assert (insets Ih = KS) as Insets_hd.
+    { rewrite /insets Dom_Ih. rewrite -leibniz_equiv_iff big_opS_singleton.
+      rewrite /Ih /inset /inf /= lookup_insert /= /ks'. 
+      rewrite nzmap_dom_insert_nonzero. rewrite Dom_ks /KS.
+      apply leibniz_equiv_iff. rewrite set_eq_subseteq. split;
+      (intros x; rewrite elem_of_union elem_of_singleton !elem_of_gset_seq; lia).
+      rewrite /ccmunit /= /nat_unit. lia. }
+    assert (dom ks = KS ∖ {[0]}) as Dom_ks2.
+    { rewrite Dom_ks /KS. apply leibniz_equiv_iff. rewrite set_eq_subseteq. 
+      split; (intros x; rewrite elem_of_difference elem_of_singleton 
+        !elem_of_gset_seq; lia). }
+    assert (outsets Ih = KS ∖ {[0]}) as Outsets_hd.
+    { rewrite /outsets Domout_Ih. rewrite -leibniz_equiv_iff big_opS_singleton.
+      rewrite /Ih /outset /out /= nzmap_lookup_total_insert. 
+      rewrite leibniz_equiv_iff. done. }
+    assert (keyset (FI s hd) = {[0]}) as KS_hd.
+    { rewrite FI_hd /keyset Insets_hd Outsets_hd. apply set_eq_subseteq. split.
+      intros x. rewrite !elem_of_difference !elem_of_singleton. 
+      intros [Hx Hx']. destruct (decide (x = 0)) as [-> | ?]; try done.
+      exfalso. apply Hx'. done. intros x. 
+      rewrite !elem_of_difference !elem_of_singleton. intros ->.
+      split. rewrite /KS elem_of_gset_seq. lia. intros ?. lia. }
+    assert (insets It = KS ∖ {[0]}) as Insets_tl.
+    { rewrite /insets Dom_It. rewrite -leibniz_equiv_iff big_opS_singleton.
+      rewrite /It /inset /inf /= lookup_insert /= /ks'. 
+      rewrite leibniz_equiv_iff. done. }
+    assert (outsets It = ∅) as Outsets_tl.
+    { rewrite /outsets Domout_It big_opS_empty. set_solver. }
+    assert (keyset (FI s tl) = KS ∖ {[0]}) as KS_tl.
+    { rewrite FI_tl /keyset Insets_tl Outsets_tl. clear; set_solver. }
+    assert (abs s = C) as Habs. { rewrite /abs /s. done. }
+    assert (FP s = {[hd; tl]}) as FP_s. { rewrite /FP /s. done. }
+    assert (Height s hd = L) as Ht_hd. 
+    { rewrite /Height /s /H lookup_insert. done. }
+    assert (Height s tl = L) as Ht_tl. 
+    { rewrite /Height /s /H lookup_insert_ne; try done.
+      rewrite lookup_insert. done. }
+    assert (Mark s hd = mh) as Mk_hd.
+    { rewrite /Mark /s /H lookup_insert. done. }
+    assert (Mark s tl = mt) as Mk_tl. 
+    { rewrite /Mark /s /H lookup_insert_ne; try done.
+      rewrite lookup_insert. done. }
+    assert (Next s hd = nh) as Nx_hd.
+    { rewrite /Next /s /H lookup_insert. done. }
+    assert (Next s tl = ∅) as Nx_tl. 
+    { rewrite /Next /s /H lookup_insert_ne; try done.
+      rewrite lookup_insert. done. }
+
+    iAssert (resources _ _ _ γ_ks s)%I with "[- Hpost]" as "Res".
+    { rewrite /resources. iFrame "HKS". rewrite FP_s.
+      rewrite !big_sepS_union. rewrite !big_sepS_singleton.
+      rewrite Ht_hd Ht_tl Key_hd Key_tl Mk_hd Mk_tl Nx_hd Nx_tl. 
+      rewrite KS_hd KS_tl Content_hd Content_tl. iFrame.
+      all: (clear -hd_neq_tl; set_solver). }
+
+    iAssert (⌜∀ n k, n ∈ FP s → k ∈ keyset (FI s n) →
+      (k ∈ abs s ↔ k ∈ Content s n)⌝)%I as "%Hks".
+    { iDestruct "Res" as "(GKS & _ & HKS)".
+      iPoseProof (keyset_summary with "GKS HKS") as "%H'"; try done. }
+    
+    assert (✓ GFI s) as Valid.
+    { rewrite /GFI FP_s big_opS_union; last first. clear -hd_neq_tl; set_solver. 
+      assert (✓ Ih) as Vh. 
+      { rewrite /valid /=. split. rewrite dom_insert_L. 
+        rewrite nzmap_dom_insert_nonzero; try done. rewrite /dom. 
+        clear -hd_neq_tl; set_solver.
+        intros H'; try done. }
+      assert (✓ It) as Vt. 
+      { rewrite /valid /=. split. rewrite dom_insert_L. rewrite /dom. 
+        clear; set_solver. intros H'; try done. }
+      rewrite !big_opS_singleton FI_hd FI_tl. apply intValid_composable.
+      split; last split; last split; last split; try done.
+      rewrite Dom_Ih Dom_It. clear -hd_neq_tl; set_solver.
+      apply map_Forall_lookup. intros n m Hm. 
+      assert (out It n = 0%CCM) as ->.
+      { rewrite /out /It /= nzmap_lookup_empty. done. }
+      rewrite ccm_pinv_unit left_id /inf Hm /=. done.
+      apply map_Forall_lookup. intros n m Hm. 
+      destruct (decide (n = tl)) as [-> | ?]; last first.
+      { rewrite /inf_map /It /= lookup_insert_ne in Hm; try done. }
+      assert (out Ih tl = ks) as ->.
+      { rewrite /out /Ih /= nzmap_lookup_total_insert. done. }
+      rewrite /inf Hm /=. rewrite /It /= lookup_insert in Hm. inversion Hm.
+      rewrite ccm_pinv_inv ccm_right_id. done. }
+    
+    assert (GFI s = Ih ⋅ It) as Def_GFI.
+    { rewrite /GFI FP_s big_opS_union; last first. clear -hd_neq_tl; set_solver. 
+      rewrite !big_opS_singleton FI_hd FI_tl. done. }
+    
+    assert (per_tick_inv hd tl s) as PT_s.
+    { split; last split; last split; last split; last split; last split.
+      - rewrite FP_s Ht_hd Ht_tl Mk_hd Mk_tl Nx_hd Nx_tl Key_hd Key_tl.
+        repeat split; try done. intros i Hi. rewrite lookup_total_alt.
+        rewrite Mh_i; try done. intros i Hi. rewrite lookup_total_alt.
+        rewrite Mt_i; try done. apply Nh_i. lia.
+      - split. done. intros n Hn. rewrite Def_GFI. 
+        destruct (decide (n = tl)) as [-> | ?]. rewrite Def_GFI in Valid.
+        assert (tl ∈ dom It) as H'. { rewrite Dom_It. clear; set_solver. }
+        pose proof intComp_inf_2 Ih It Valid tl H' as H''. rewrite H''.
+        rewrite /inf /It /Ih /out /= lookup_insert nzmap_lookup_total_insert /=.
+        rewrite ccm_pinv_inv. done. rewrite /inf.
+        destruct (inf_map (Ih ⋅ It) !! n) eqn: H'; try done. 
+        rewrite Def_GFI in Valid.
+        apply flowint_contains in H'; try done. rewrite intComp_dom in H'; try done.
+        rewrite Dom_Ih Dom_It in H'. clear -Hn n0 H'; set_solver.
+      - apply Hks.
+      - intros n. rewrite FP_s elem_of_union !elem_of_singleton. intros [-> | ->].
+        + rewrite Ht_hd Mk_hd Nx_hd Key_hd FI_hd. 
+          split; last split; last split; last split; last split; try done.
+          * intros _. rewrite lookup_total_alt Mh_i; try done. lia.
+          * lia.
+          * rewrite Nh_i; try done. rewrite lookup_total_alt Mh_i /=; try done.
+            repeat split; try done. rewrite Outsets_hd Insets_hd. clear; set_solver.
+            rewrite Insets_hd /KS. done. rewrite Outsets_hd /= -Dom_ks2 Dom_ks. done.
+            intros _. rewrite Insets_hd /KS elem_of_gset_seq. lia.
+            intros k. rewrite Insets_hd /KS elem_of_gset_seq. clear; lia.
+            intros k. rewrite /inf /Ih /= lookup_insert /= /ks'.
+            destruct (decide (k = 0)) as [-> | ?]; try done.
+            rewrite nzmap_lookup_total_insert. done. 
+            rewrite nzmap_lookup_total_insert_ne; try done.  
+            intros n k. rewrite /out /Ih /=. destruct (decide (n = tl)) as [-> | ?].
+            rewrite nzmap_lookup_total_insert. done.
+            rewrite nzmap_lookup_total_insert_ne; try done. 
+            rewrite nzmap_lookup_empty /ccmunit /= /nat_unit. clear; lia.
+            all : (clear -HL; lia).
+        + rewrite Ht_tl Mk_tl Nx_tl Key_tl FI_tl. 
+          split; last split; last split; last split; last split; try done.
+          * intros _. rewrite lookup_total_alt Mt_i; try done. lia.
+          * lia.
+          * rewrite lookup_total_alt Mt_i /=; last first. lia.
+            rewrite lookup_empty. repeat split; try done.
+            rewrite Outsets_tl Insets_tl. clear; set_solver.
+            rewrite Insets_tl /KS. intros x. rewrite elem_of_difference !elem_of_gset_seq.
+            rewrite elem_of_singleton. clear -HW; lia.
+            rewrite Outsets_tl. apply set_eq_subseteq. split.
+            intros x. rewrite elem_of_gset_seq. clear; lia. clear; set_solver.
+            intros _. rewrite Insets_tl /KS elem_of_difference elem_of_gset_seq.
+            rewrite elem_of_singleton. clear -HW; lia.
+            intros k. rewrite Insets_tl /KS elem_of_difference elem_of_gset_seq.
+            rewrite elem_of_singleton; clear; lia.
+            intros k. rewrite /inf /It /= lookup_insert /= /ks'. done.
+            intros n k. rewrite /out /It /=.
+            rewrite !nzmap_lookup_empty /ccmunit /= /nat_unit. clear; lia.
+      - intros n1 n2 Hnx. destruct (decide (n1 = hd)) as [-> | ?].
+        + rewrite /Nexti Nx_hd Nh_i in Hnx; try done. inversion Hnx. subst n2.
+          rewrite Key_hd Key_tl. done. lia.
+        + rewrite /Nexti /s /Next /Nx lookup_insert_ne in Hnx.
+          destruct (decide (n1 = tl)) as [-> | ?].
+          rewrite lookup_insert lookup_empty in Hnx. done.
+          rewrite lookup_insert_ne in Hnx. rewrite lookup_empty in Hnx. done.
+          all: try done.
+      - intros n1 n2 i Hnx. destruct (decide (n1 = hd)) as [-> | ?].
+        + assert (i < L) as H'. { rewrite /Nexti Nx_hd in Hnx. 
+          apply elem_of_dom_2 in Hnx. rewrite Dom_nh elem_of_gset_seq in Hnx. lia. }
+          rewrite /Nexti Nx_hd Nh_i in Hnx; try done. inversion Hnx. subst n2.
+          rewrite FP_s. clear; set_solver.
+        + rewrite /Nexti /s /Next /Nx lookup_insert_ne in Hnx.
+          destruct (decide (n1 = tl)) as [-> | ?].
+          rewrite lookup_insert lookup_empty in Hnx. done.
+          rewrite lookup_insert_ne in Hnx. rewrite lookup_empty in Hnx. done.
+          all: try done.
+      - intros n1 n2 i Hnx. destruct (decide (n1 = hd)) as [-> | ?].
+        + assert (i < L) as H'. { rewrite /Nexti Nx_hd in Hnx. 
+          apply elem_of_dom_2 in Hnx. rewrite Dom_nh elem_of_gset_seq in Hnx. lia. }
+          rewrite /Nexti Nx_hd Nh_i in Hnx; try done. inversion Hnx. subst n2.
+          rewrite Ht_tl; lia.
+        + rewrite /Nexti /s /Next /Nx lookup_insert_ne in Hnx.
+          destruct (decide (n1 = tl)) as [-> | ?].
+          rewrite lookup_insert lookup_empty in Hnx. done.
+          rewrite lookup_insert_ne in Hnx. rewrite lookup_empty in Hnx. done.
+          all: try done. }
+    
+    iModIntro. iApply ("Hpost" $! r s). iExists hd, tl, γ_ks. iFrame "#∗%".
+    iPureIntro. split. intros t Ht. assert (t = 0) as -> by lia.
+    rewrite lookup_total_insert. done.
+    intros t Ht. clear -Ht; lia.
+  Qed.
   
-  Lemma dsOp_spec (Σ : gFunctors) (H' : heapGS Σ) (H'' : dsG Σ) (H''' : hsG Σ)
-    N γ_t γ_r γ_m γ_mt γ_msy r op (p: proph_id) pvs tid t0 Q :
-          main_inv Σ H' H'' H''' N γ_t γ_r γ_m γ_mt γ_msy r -∗
-          thread_start Σ H' H'' H''' γ_t γ_mt tid t0 -∗
-          □ update_helping_protocol Σ H' H'' H''' N γ_t γ_r γ_mt γ_msy -∗
+  Lemma dsOp_spec Σ Hg1 Hg2 Hg3 N γ_t γ_r γ_m γ_mt γ_msy r op (p: proph_id) 
+    pvs tid t0 Q :
+          main_inv Σ Hg1 Hg2 Hg3 N γ_t γ_r γ_m γ_mt γ_msy r -∗
+          thread_start Σ Hg1 Hg2 Hg3 γ_t γ_mt tid t0 -∗
+          □ update_helping_protocol Σ Hg1 Hg2 Hg3 N γ_t γ_r γ_mt γ_msy -∗
           ⌜local_pre op⌝ -∗
             {{{ proph p pvs ∗ 
                 (match process_proph tid pvs with
-                  contra => au Σ H' H'' H''' N γ_r op Q
+                  contra => au Σ Hg1 Hg2 Hg3 N γ_r op Q
                 | no_upd => True
-                | upd => au Σ H' H'' H''' N γ_r op Q end) }}}
+                | upd => au Σ Hg1 Hg2 Hg3 N γ_r op Q end) }}}
                   dsOp (Op_to_val op) #p #r @ ⊤
             {{{ (res: resT) prf pvs', RET #res;
                 proph p pvs' ∗ ⌜pvs = prf ++ pvs'⌝ ∗
                 (match process_proph tid pvs with
                   contra => ⌜Forall (λ x, x.2 ≠ #tid) prf⌝
-                | no_upd => past_lin_witness Σ H' H'' H''' γ_m op res t0
+                | no_upd => past_lin_witness Σ Hg1 Hg2 Hg3 γ_m op res t0
                 | upd => Q #res ∨ 
                     ⌜Forall (λ x, ¬ is_snd true x ∧ x.2 ≠ #tid) prf⌝ end) }}}.
   Proof.
@@ -46,9 +330,9 @@ Module SKIPLIST_SPEC : HINDSIGHT_SPEC.
     iIntros (Φ) "!# Hpre Hpost". 
     wp_lam. wp_pures. wp_bind (! _)%E.
     iInv "HInv" as (M0 T0 s0) "(>Ds & >%Habs0 & >Hist & Help & >Templ)".
-    iDestruct "Templ" as (hd tl)"(#HR & SShot0 & Res & %PT0 & %Trans_M0)".
+    iDestruct "Templ" as (hd tl γ_ks)"(#HR & SShot0 & Res & %PT0 & %Trans_M0)".
     wp_load. iModIntro. iSplitR "Hpre Hpost".
-    { iExists M0, T0, s0. iNext. iFrame "%#∗". iExists hd, tl. iFrame "%#". }
+    { iExists M0, T0, s0. iNext. iFrame "%#∗". iExists hd, tl, γ_ks. iFrame "%#∗". }
     wp_pures. unfold Op_to_val; destruct op as [k|k|k]; wp_pures.
     - wp_apply (SK_SEARCH.searchOp_spec with "[] [] [] [] [] [Hpre]"); try done.
     - wp_apply (SK_INSERT.insertOp_spec with "[] [] [] [] [] [Hpre]"); try done.
